- kind compilation - type compilation complete - typing and kinding judgments uniqueness - defining substitution and weakening over compile and HsJudgments

Hs/Algorithm.lean
@@ -1,6 +1,7 @@
 import Hs.HsJudgment
 import Hs.HsTerm
 import SystemFD.Term
+import SystemFD.Algorithm
 
 def compile_kind (Γ : Ctx HsTerm) (κ : HsTerm) (ty : HsTerm) : Γ ⊢κ κ : ty -> Option Term
 | .ax _ => some ★
@@ -13,8 +14,13 @@ def compile_type (Γ : Ctx HsTerm) (τ : HsTerm) (k : HsTerm) : Γ ⊢τ τ : k 
 -----------------------------
 ----- Types and kinds
 -----------------------------
-| @HsJudgment.varTy _ x _ _ _ _ => .some #x
-| @HsJudgment.appk Γ f A B a j1 j2 => do
+-- TODO: What if we just return the compiled type with the compiled term?
+| @HsJudgment.varTy _ x T _ _ _ j => do
+  let _ <- compile_kind Γ T `□ j
+  .some #x
+| @HsJudgment.appk Γ f A B a j1 j2 j3 j4 => do
+  let _ <- compile_kind Γ A `□ j3
+  let _ <- compile_kind Γ B `□ j4
   let t1 <- compile_type Γ f (A `-k> B) j1
   let t2 <- compile_type Γ a A j2
   .some (t1 `@k t2)
@@ -60,9 +66,11 @@ def compile_term (Γ : Ctx HsTerm) (t : HsTerm) (τ : HsTerm) : Γ ⊢t t : τ -
 ----------------------------------------
 --- Implicit
 ----------------------------------------
-| @HsJudgment.implicitAllE Γ t A τ e j1 j2  => do
-  let t1 <- (compile_term Γ t (`∀{A}τ) j1)
-  let t2 <- (compile_term Γ e A j2)
+| @HsJudgment.implicitAllE Γ A τ t e j1 j2 j3 j4 => do
+  let _ <- compile_type Γ (`∀{A}τ) `★ j1
+  let _ <- compile_kind Γ A `□ j2
+  let t1 <- (compile_term Γ t (`∀{A}τ) j3)
+  let t2 <- (compile_type Γ e A j4)
   .some (t1 `@t t2)
 | @HsJudgment.implicitAllI Γ A t τ j1 j2 j3 => do
   let t' <- compile_term (.kind A :: Γ) t τ j1
@@ -82,36 +90,42 @@ termination_by h => h.size
 inductive HsCtx : Ctx HsTerm -> Type where
 | nil : HsCtx []
 | empty : HsCtx Γ -> HsCtx (.empty::Γ)
-| kind : HsCtx Γ -> (k : HsTerm) × (Γ ⊢κ k : `□) -> HsCtx (.kind k :: Γ)
-| datatype : HsCtx Γ -> (k : HsTerm) × (Γ ⊢κ k : `□) -> HsCtx (.datatype k :: Γ)
-| type : HsCtx Γ -> (τ : HsTerm) × (Γ ⊢τ τ : `★) -> HsCtx (.type τ :: Γ)
-| ctor : HsCtx Γ -> (τ : HsTerm) × (Γ ⊢τ τ : `★) -> HsCtx (.ctor τ :: Γ)
-| openm : HsCtx Γ -> (τ : HsTerm) × (Γ ⊢τ τ : `★) -> HsCtx (.openm τ :: Γ)
+| kind : HsCtx Γ -> (Γ ⊢κ k : `□) -> HsCtx (.kind k :: Γ)
+| datatype : HsCtx Γ -> (Γ ⊢κ k : `□) -> HsCtx (.datatype k :: Γ)
+| type : HsCtx Γ -> (Γ ⊢τ τ : `★) -> HsCtx (.type τ :: Γ)
+| ctor : HsCtx Γ -> (Γ ⊢τ τ : `★) -> HsCtx (.ctor τ :: Γ)
+| openm : HsCtx Γ -> (Γ ⊢τ τ : `★) -> HsCtx (.openm τ :: Γ)
 
 @[simp]
 def compile_ctx : HsCtx Γ -> Option (Ctx Term)
 | .nil => .some []
 | .empty Γ => do
-  let Γ' <- compile_ctx Γ
-  .some (.empty :: Γ')
-| @HsCtx.kind Γ _ Γ' ⟨t, j⟩ => do
+  let Δ <- compile_ctx Γ
+  let _ <- wf_ctx Δ
+  .some (.empty :: Δ)
+| @HsCtx.kind Γ k Γ' j => do
   let Δ <- compile_ctx Γ'
-  let τ <- compile_kind Γ t `□ j
+  let _ <- wf_ctx Δ
+  let τ <- compile_kind Γ k `□ j
   .some (.kind τ :: Δ)
-| @HsCtx.datatype Γ _ Γ' ⟨t, j⟩ => do
+| @HsCtx.datatype Γ t Γ' j => do
   let Δ <- compile_ctx Γ'
+  let _ <- wf_ctx Δ
   let τ <- compile_kind Γ t `□ j
   .some (.datatype τ :: Δ)
-| @HsCtx.type Γ _ Γ' ⟨t, j⟩ => do
+| @HsCtx.type Γ t Γ' j => do
   let Δ <- compile_ctx Γ'
+  let _ <- wf_ctx Δ
   let τ <- compile_type Γ t `★ j
   .some (.type τ :: Δ)
-| @HsCtx.ctor Γ _ Γ' ⟨t, j⟩ => do
+| @HsCtx.ctor Γ t Γ' j => do
   let Δ <- compile_ctx Γ'
+  let _ <- wf_ctx Δ
   let τ <- compile_type Γ t `★ j
   .some (.ctor τ :: Δ)
-| @HsCtx.openm Γ _ Γ' ⟨t, j⟩ => do
+| @HsCtx.openm Γ t Γ' j => do
   let Δ <- compile_ctx Γ'
+  let _ <- wf_ctx Δ
   let τ <- compile_type Γ t `★ j
   .some (.openm τ :: Δ)
 
