Hs/Metatheory/Preservation2.lean
@@ -1,7 +1,10 @@
 import Hs.Algorithm
 import Hs.Metatheory.Uniqueness
-
-import Aesop
+import Hs.Metatheory.Weaken
+import Hs.Metatheory.WeakenCompile
+import Hs.Metatheory.Substitution
+import Hs.Metatheory.SubstitutionCompile
+import SystemFD.Algorithm.Soundness2
 
 set_option maxHeartbeats 500000
 
@@ -21,6 +24,13 @@ inductive CompileCtx : Ctx HsTerm -> Ctx Term -> Prop where
   (j1 : Γ ⊢κ A : `□) ->
   compile_kind Γ A `□ j1 = .some A' ->
   CompileCtx (.kind A :: Γ) (.kind A' :: Γ')
+| datatype :
+  ⊢s Γ ->
+  ⊢ Γ' ->
+  CompileCtx Γ Γ' ->
+  (j1 : Γ ⊢κ A : `□) ->
+  compile_kind Γ A `□ j1 = .some A' ->
+  CompileCtx (.datatype A :: Γ) (.datatype A' :: Γ')
 | type :
   ⊢s Γ ->
   ⊢ Γ' ->
@@ -28,6 +38,13 @@ inductive CompileCtx : Ctx HsTerm -> Ctx Term -> Prop where
   (j1 : Γ ⊢τ A : `★) ->
   compile_type Γ A `★ j1 = .some A' ->
   CompileCtx (.type A :: Γ) (.type A' :: Γ')
+| ctor :
+  ⊢s Γ ->
+  ⊢ Γ' ->
+  CompileCtx Γ Γ' ->
+  (j1 : Γ ⊢τ A : `★) ->
+  compile_type Γ A `★ j1 = .some A' ->
+  CompileCtx (.ctor A :: Γ) (.ctor A' :: Γ')
 | term :
   ⊢s Γ ->
   ⊢ Γ' ->
@@ -37,6 +54,45 @@ inductive CompileCtx : Ctx HsTerm -> Ctx Term -> Prop where
   compile_type Γ A `★ j = .some A' ->
   compile_term Γ t τ j2 = .some t' ->
   CompileCtx (.term A t :: Γ) (.term A' t' :: Γ')
+| openm :
+  ⊢s Γ ->
+  ⊢ Γ' ->
+  CompileCtx Γ Γ' ->
+  (j1 : Γ ⊢τ A : `★) ->
+  compile_type Γ A `★ j1 = .some A' ->
+  CompileCtx (.openm A :: Γ) (.openm A' :: Γ')
+
+theorem ctx_shift (Γ : Ctx HsTerm) :
+  (f :: Γ)d@(n + 1) = .datatype k ->
+  ∃ k', (Γ d@ n) = .datatype k' := by
+intro h;
+unfold dnth at h; unfold Frame.apply at h;
+generalize fh : Γ d@n = f at *;
+cases f;
+all_goals (simp at h)
+case _ a => exists a
+
+theorem compile_ctx_shape :
+  CompileCtx Γ Γ' ->
+  (Γ d@ x) = .datatype k ->
+  ∃ k', (Γ' d@ x) = .datatype k' := by
+intro cc h;
+induction cc;
+case _ => cases h
+case _ Γ Γ' wf wf' cc ih =>
+  cases x;
+  case _ => unfold dnth at h; cases h
+  case _ =>
+    have lem := ctx_shift Γ h
+    cases lem; case _ lem =>
+    sorry
+case _ => sorry
+case _ => sorry
+case _ => sorry
+case _ => sorry
+case _ => sorry
+case _ => sorry
+
 
 theorem compile_preserves_kinds :
   ⊢ Γ' ->
@@ -49,8 +105,7 @@ theorem compile_preserves_kinds :
  case _ =>
    unfold compile_kind at c; cases c;
    case _ =>
-     apply Judgment.ax;
-     assumption;
+     apply Judgment.ax; assumption;
  case _ j1 j2 ih1 ih2 =>
    unfold compile_kind at c; simp at c;
    rw[Option.bind_eq_some] at c;
@@ -66,58 +121,136 @@ theorem compile_preserves_kinds :
    apply ih1';
    apply ih2'
 
-def wf_ctx_well_kinded_types : ⊢s Γ -> (Γ d@ x).is_datatype -> (Γ d@ x).get_type = .some T ->  Γ ⊢κ T : `□ := sorry
+theorem compile_preserves_kind_indices :
+  (∀ Γ (h1 h2 : ⊢s Γ), h1 = h2) ->
+  CompileCtx Γ Γ' ->
+  (Γ d@ x).is_datatype || (Γ d@ x).is_kind ->
+  (j : Γ ⊢κ k : s) ->
+  (Γ d@ x).get_type = .some k ->
+  compile_kind Γ k s j = .some k' ->
+  (Γ' d@ x).get_type = .some k' := by
+intro h' cc t j gt c;
+sorry
+-- induction Γ, k, s, j using compile_kind.induct generalizing k'
+-- case _ Γ wf =>
+--   unfold compile_kind at c; cases c;
+--   induction cc generalizing x <;> simp at *
+--   case _ =>
+--     cases t;
+--     case _ t => cases t
+--     case _ t => cases t
+--   case _ ih =>
+--     cases t;
+--     case _ t =>
+--       cases wf; case _ wf =>
+--       have ih' := @ih (x - 1) sorry sorry sorry
+--       sorry
+--     case _ => sorry
+--   case _ => sorry
+--   case _ => sorry
+--   case _ => sorry
+--   case _ => sorry
+-- case _ => sorry
 
-def typing_implies_kinding : ∀ Γ, Γ ⊢τ τ : κ -> Γ ⊢κ κ : `□
-| Γ, .varTy wf c gt => sorry
-| Γ, .appk h _ => sorry
-| Γ, .allt h _ =>  HsJudgment.ax (hs_judgment_ctx_wf .kind h)
-| Γ, .arrow h _ => HsJudgment.ax (hs_judgment_ctx_wf .type h)
-| Γ, .farrow h _ _ => HsJudgment.ax (hs_judgment_ctx_wf .type h)
 
+
+-- have lem := well_sorted_kind_inversion j; cases lem
+-- induction x generalizing Γ Γ' <;> simp at *;
+-- case _ =>
+--   unfold Frame.get_type at gt;
+--   cases t;
+--   case _ h =>
+--     have lem := datatype_indexing_exists h;
+--     cases lem; case _ w h =>
+--     rw [h] at gt; simp at gt; cases gt; unfold Frame.get_type;
+--     cases cc <;> cases h; unfold dnth; unfold Frame.apply; simp;
+--     case _ wf wf' cc ja ca =>
+--     have lem1 := hs_weaken_kind (HsJudgment.wfdatatype ja wf) ja
+--     have lem2 := weaken_compile_kind ja lem1 ca
+--     apply compile_kind_uniqueness h' lem1 j lem2 c;
+--   case _ h =>
+--     have lem := kind_indexing_exists h;
+--     cases lem; case _ w h =>
+--     rw [h] at gt; simp at gt; cases gt; unfold Frame.get_type;
+--     cases cc <;> cases h; unfold dnth; unfold Frame.apply; simp;
+--     case _ wf wf' cc ja ca =>
+--     have lem1 := hs_weaken_kind (HsJudgment.wfkind ja wf) ja
+--     have lem2 := weaken_compile_kind ja lem1 ca
+--     apply compile_kind_uniqueness h' lem1 j lem2 c;
+-- case _ ih =>
+--   have ih' := @ih (.empty :: Γ) (.empty :: Γ')
+--   sorry
+
+
+-- theorem compile_preserves_kind_shape :
+--   ⊢ Γ' ->
+--   (∀ Γ (h1 h2 : ⊢s Γ), h1 = h2) ->
+--   (j1 : Γ ⊢κ A : `□) ->
+--   (j2 : Γ ⊢κ B : `□) ->
+--   (j3 : Γ ⊢κ (A `-k> B) : `□) ->
+--   compile_kind Γ A `□ j1 = .some A' ->
+--   compile_kind Γ B `□ j2 = .some B' ->
+--   compile_kind Γ (A `-k> B) `□ j3 = .some t' ->
+--   t' = (A' -k> B') := by
+-- intro wf h j1 j2 j3 c1 c2 c3;
+-- have c3' := c3;
+-- unfold compile_kind at c3; cases j3;
+-- case _ ja jb =>
+-- simp at c3;
+-- rw[Option.bind_eq_some] at c3;
+-- cases c3; case _ w1 c3 =>
+-- cases c3; case _ c3 c4 =>
+-- rw[Option.bind_eq_some] at c4;
+-- cases c4; case _ w2 c4 =>
+-- cases c4; case _ c4 c5 =>
+-- cases c5;
+-- have u := kinds_compiling_uniqueness h j1 ja c1 c3; cases u;
+-- have u := kinds_compiling_uniqueness h j2 jb c2 c4; cases u;
+-- simp
 
 theorem compile_preserves_types :
   CompileCtx Γ Γ' ->
   ⊢ Γ' ->
+  (∀ Γ (h1 h2 : ⊢s Γ), h1 = h2) ->
   (j2 : Γ ⊢κ k : `□) ->
   compile_kind Γ k `□ j2 = .some k' ->
   (j1 : Γ ⊢τ τ : k) ->
   compile_type Γ τ k j1 = .some τ' ->
   Γ' ⊢ τ' : k' := by
-intro cc wf j1 c1 j2 c2;
+intro cc wf h j1 c1 j2 c2;
 induction Γ, τ, k, j2 using compile_type.induct generalizing Γ' τ' k'
 all_goals (unfold compile_type at c2; simp at c2)
 case _ Γ x wf test gt =>
      cases c2;
-     apply Judgment.var;
-     assumption;
-
-     sorry
-  -- apply compile_ctx_wf; assumption; assumption;
-  -- have lem1 := HsJudgment.varTy wf test gt
-  -- have lem := compile_preserves_type_indices cc lem1 c1; symm at lem;
-  -- assumption
-case _ B Γ f A a h1 h2 ih1 ih2 =>
+     have lem := Eq.symm (compile_preserves_kind_indices h cc test j1 (Eq.symm gt) c1)
+     apply Judgment.var; assumption; assumption
+case _ B Γ f A a h1 h2 ja jb ih1 ih2 =>
   rw[Option.bind_eq_some] at c2;
   cases c2; case _ w1 c2 =>
   cases c2; case _ c2 c3 =>
   rw[Option.bind_eq_some] at c3;
   cases c3; case _ w2 c3 =>
-  cases c3; case _ c3 e =>
+  cases c3; case _ c3 c4 =>
+  rw[Option.bind_eq_some] at c4;
+  cases c4; case _ w3 c4 =>
+  cases c4; case _ c4 c5 =>
+  rw[Option.bind_eq_some] at c5;
+  cases c5; case _ w4 c5 =>
+  cases c5; case _ c5 e =>
   cases e;
   apply Judgment.appk;
   case _ =>
-    apply @ih1 Γ' _ w1 cc wf _ _ c2
-    case _ => sorry
-    case _ =>
-      apply HsJudgment.arrowk;
-      apply typing_implies_kinding Γ h2;
-      assumption
-    case _ => sorry
+    have u := compile_kind_uniqueness h j1 jb c1 c3; cases u;
+    have h' : compile_kind Γ (A `-k> B) `□ (ja.arrowk jb) = some (w1 -k> k') := by
+      unfold compile_kind; simp;
+      rw[Option.bind_eq_some];
+      exists w1; apply And.intro
+      case _ => assumption
+      case _ => rw[Option.bind_eq_some]; simp; assumption
+    have ih1' := @ih1 Γ' (w1 -k> k') w3 cc wf (HsJudgment.arrowk ja jb) h' c4
+    apply ih1';
   case _ =>
-    apply @ih2 Γ' _ w2 cc wf _ _ c3
-    case _ => apply typing_implies_kinding Γ h2;
-    case _ => sorry
+    apply @ih2 Γ' w1 w4 cc wf ja c2 c5
 
 case _ h1 h2 ih1 =>
   rw[Option.bind_eq_some] at c2;
@@ -180,25 +313,69 @@ case _ j1 _ j2 ih1 ih2 =>
   case _ => apply HsJudgment.ax; apply HsJudgment.wfempty; assumption
   case _ => unfold compile_kind; rfl
 
+@[simp]
+abbrev CompilePreservesTypeShapeAll :  (v : HsVariant) -> Ctx HsTerm -> HsJudgmentArgs v -> Prop
+| .type => λ Γ => λ (τ, k) => ∀ wA wτ cτ,
+  τ = (`∀{wA} wτ) ->
+  k = `★ ->
+  (j3 : Γ ⊢τ τ : k) ->
+  compile_type Γ τ k j3 = .some cτ ->
+  ∃ A' τ', cτ = ∀[A']τ'
+| _ => λ _ => λ _ => true
+
+theorem comile_preserves_type_shape_all_lemma :
+  HsJudgment v Γ idx -> CompilePreservesTypeShapeAll v Γ idx
+ := by
+intro j; induction j <;> simp at *;
+intro wA wτ cτ e1 e2 j3 c3;
+cases j3; case _ hka hkb =>
+unfold compile_type at c3; simp at c3;
+rw[Option.bind_eq_some] at c3;
+cases c3; case _ A' c3 =>
+cases c3; case _ cA c4 =>
+rw[Option.bind_eq_some] at c4;
+cases c4; case _ B' c4 =>
+cases c4; case _ cB e =>
+cases e; simp;
+
+theorem compile_preserves_type_shape_all :
+  (j : Γ ⊢τ (`∀{A}τ) : `★) ->
+  compile_type Γ (`∀{A}τ) `★ j = .some cτ ->
+  ∃ A' τ', cτ = ∀[A']τ' := by
+intro j c;
+have lem := comile_preserves_type_shape_all_lemma j; simp at lem;
+apply @lem A τ cτ rfl rfl j c
+
+
+theorem compile_preserves_type_indices :
+  (∀ Γ (h1 h2 : ⊢s Γ), h1 = h2) ->
+  CompileCtx Γ Γ' ->
+  (Γ d@ x).is_ctor || (Γ d@ x).is_term || (Γ d@ x).is_type ->
+  (j : Γ ⊢τ T : k) ->
+  (Γ d@ x).get_type = .some T ->
+  compile_type Γ T k j = .some T' ->
+  (Γ' d@ x).get_type = .some T' := by sorry
+
 theorem compile_preserves_terms :
   (∀ Γ (h1 h2 : ⊢s Γ), h1 = h2) ->
+  CompileCtx Γ Γ' ->
   ⊢ Γ' ->
   (j1 : Γ ⊢τ τ : k) ->
   compile_type Γ τ k j1 = .some τ' ->
   (j2 : Γ ⊢t t : τ) ->
   compile_term Γ t τ j2 = .some t' ->
   Γ' ⊢ t' : τ' := by
-intro h cc j1 c1 j2 c2;
+intro h cc wf j1 c1 j2 c2;
 induction Γ, t, τ, j2 using compile_term.induct generalizing Γ' t' τ' k
 all_goals (unfold compile_term at c2; simp at c2)
-case _ wf test gt => sorry
-  -- cases c2;
-  -- have lem1 := HsJudgment.var wf test gt
-  -- have lem := compile_preserves_term_indices cc lem1 c1
-  -- apply Judgment.var;
-  -- apply compile_ctx_wf wf cc
-  -- sorry
-case _ j1' j2 j3 ih1 =>
+case _ wf test gt =>
+     cases c2;
+     apply Judgment.var;
+     assumption;
+     have lem := compile_preserves_type_indices h cc test j1 (Eq.symm gt) c1;
+     apply Eq.symm lem
+
+case _ Γ A t B j1' j2 j3 ih1 => -- lam
  rw[Option.bind_eq_some] at c2;
  cases c2; case _ A' c2 =>
  cases c2; case _ c2 c3 =>
@@ -214,64 +391,314 @@ case _ j1' j2 j3 ih1 =>
  rw[Option.bind_eq_some] at c2';
  cases c2'; case _ B' c2' =>
  cases c2'; case _ c2' e =>
- cases e;
- have e : x1 = A' := by
+ cases e; case _ ja jb =>
+ have lem := compile_type_uniqueness h j1' ja c2 c1'; cases lem;
+ apply Judgment.lam;
+ apply compile_preserves_types cc wf h _ _ ja c1'
+ case _ => apply HsJudgment.ax (hs_judgment_ctx_wf .type ja)
+ case _ => unfold compile_kind; rfl
+ case _ =>
+   have ih1' := @ih1 (.type A' :: Γ') `★ B' t'
    sorry
- have ih1' := @ih1 (.type A' :: Γ') `★ B' t' sorry sorry sorry c3
+ apply compile_preserves_types cc wf h _ _ _ _
+ case _ => apply `★;
+ case _ => apply (A → B)
+ case _ => apply HsJudgment.ax (hs_judgment_ctx_wf .type ja)
+ case _ => unfold compile_kind; rfl
+ case _ => apply HsJudgment.arrow; assumption; assumption
+ case _ =>
+   unfold compile_type; simp;
+   rw[Option.bind_eq_some]; exists A';
+   apply And.intro; assumption;
+   rw[Option.bind_eq_some]; exists B';
 
+
+case _ h1 h2 ih1 ih2 =>
+ rw[Option.bind_eq_some] at c2;
+ cases c2; case _ wt1 c2 =>
+ cases c2; case _ c2 c3 =>
+ rw[Option.bind_eq_some] at c3;
+ cases c3; case _ wt2 c3 =>
+ cases c3; case _ c3 e =>
+ cases e;
+ apply Judgment.app;
+ sorry
+ case _ =>
+   have ih2' := @ih2 Γ' `★
+   sorry
+ sorry
+ sorry
  sorry
 
-case _ =>
- sorry
 case _ =>
  sorry
 case _ =>
  sorry
 
 -- implicits
-case _ => sorry
+case _ Γ t A τ e h1 h2 h3 h4 ih => -- implicitAllE
+ rw[Option.bind_eq_some] at c2;
+ cases c2; case _ wτ c2 =>
+ cases c2; case _ c2 c3 =>
+ rw[Option.bind_eq_some] at c3;
+ cases c3; case _ wA c3 =>
+ cases c3; case _ c3 c4 =>
+ rw[Option.bind_eq_some] at c4;
+ cases c4; case _ wt c4 =>
+ cases c4; case _ c4 c5 =>
+ rw[Option.bind_eq_some] at c5;
+ cases c5; case _ we c5 =>
+ cases c5; case _ c5 e =>
+ cases e;
+ have lem := compile_preserves_type_shape_all h1 c2;
+ cases lem; case _ A' lem =>
+ cases lem; case _ τ' lem =>
+ cases lem;
+ apply Judgment.appt;
+ case _ => --
+   have ih' := @ih Γ' `★ (∀[A']τ') wt cc wf h1 c2 c4;
+   apply ih'
+ case _ =>
+   have h' := compile_preserves_types cc wf h h2 c3 h4 c5
+   unfold compile_type at c2; cases h1; simp at c2;
+   rw[Option.bind_eq_some] at c2;
+   cases c2; case _ wA' c2' =>
+   cases c2'; case _ c2' c3' =>
+   rw[Option.bind_eq_some] at c3';
+   cases c3'; case _ wτ' c3' =>
+   cases c3'; case _ c3' e  =>
+   cases e; case _ h2' _ =>
+   have lem := compile_kind_uniqueness h h2 h2' c3 c2'; cases lem;
+   assumption
+ case _ =>
+   have h' := compile_preserves_types cc wf h h2 c3 h4 c5
+   unfold compile_type at c2; cases h1; simp at c2;
+   rw[Option.bind_eq_some] at c2;
+   cases c2; case _ wA' c2' =>
+   cases c2'; case _ c2' c3' =>
+   rw[Option.bind_eq_some] at c3';
+   cases c3'; case _ wτ' c3' =>
+   cases c3'; case _ c3' e  =>
+   cases e; case _ h2' j1' =>
+   have lem := compile_kind_uniqueness h h2 h2' c3 c2'; cases lem;
+   have j1'' := hs_beta_kind_type j1' h4; simp at j1'';
+   have u := types_have_unique_kinds j1 j1''; cases u;
+   have u := types_have_unique_judgments h j1 j1''; cases u;
+   have lem := compile_beta_kind_type j1' c3' h4 c5 j1'';
+   have lem1 : compile_type Γ ([Subst.Action.su e::I]τ) ([Subst.Action.su e::I]`★) j1'' = compile_type Γ ([Subst.Action.su e::I]τ) `★ j1'' := by rfl
+   rw[lem1] at lem;
+   rw[c1] at lem; cases lem; rfl
+
 case _ => sorry
 case _ => sorry
 case _ => sorry
 
+---------------------------------------------
+-- Contexts
+--------------------------------------------
 
-theorem compile_ctx_wf :
-  ⊢s Γ ->
-  (c : HsCtx Γ) ->
-  compile_ctx c = .some Γ' ->
-  ⊢ Γ' :=
-by
-intro h1 h2; sorry
--- induction h2;
--- case _ => apply Judgment.wfnil
--- case _ ih1 =>
---   case _ h1 =>
---   apply Judgment.wfempty; assumption;
--- case _ h1 j1 cc ih =>
---  apply Judgment.wfkind;
---  sorry
---  sorry
+theorem compile_preserves_wf Γ : ⊢s Γ -> (Η : HsCtx Γ) -> compile_ctx Η = .some Γ' -> ⊢ Γ' := by
+intro wf h cc;
+induction h generalizing Γ';
+case _ =>
+  unfold compile_ctx at cc; cases cc;
+  apply Judgment.wfnil;
+case _ ih =>
+  cases wf; case _ wf =>
+  unfold compile_ctx at cc; simp at cc;
+  rw[Option.bind_eq_some] at cc;
+  cases cc; case _ w cc =>
+  cases cc; case _ cc cc1 =>
+  rw[Option.bind_eq_some] at cc1;
+  cases cc1; case _ w1 cc1 =>
+  cases cc1; case _ cc1 cc2 =>
+  cases cc2;
+  apply Judgment.wfempty;
+  apply wf_ctx_sound cc1;
+case _ j ih =>
+  cases wf; case _ wf jk =>
+  unfold compile_ctx at cc; simp at cc;
+  rw[Option.bind_eq_some] at cc;
+  cases cc; case _ w cc =>
+  cases cc; case _ cc cc1 =>
+  rw[Option.bind_eq_some] at cc1;
+  cases cc1; case _ w1 cc1 =>
+  cases cc1; case _ cc1 cc2 =>
+  rw[Option.bind_eq_some] at cc2;
+  cases cc2; case _ w2 cc2 =>
+  cases cc2; case _ cc2 cc3 =>
+  cases cc3; cases w1;
+  apply Judgment.wfkind;
+  apply compile_preserves_kinds _ j cc2;
+  case _ => apply @ih w wf cc
+  apply @ih w wf cc
+case _ j ih =>
+  cases wf; case _ wf jk =>
+  unfold compile_ctx at cc; simp at cc;
+  rw[Option.bind_eq_some] at cc;
+  cases cc; case _ w cc =>
+  cases cc; case _ cc cc1 =>
+  rw[Option.bind_eq_some] at cc1;
+  cases cc1; case _ w1 cc1 =>
+  cases cc1; case _ cc1 cc2 =>
+  rw[Option.bind_eq_some] at cc2;
+  cases cc2; case _ w2 cc2 =>
+  cases cc2; case _ cc2 cc3 =>
+  cases cc3; cases w1;
+  apply Judgment.wfdatatype;
+  apply compile_preserves_kinds _ j cc2;
+  case _ => apply @ih w wf cc
+  apply @ih w wf cc
+case _ j ih =>
+  cases wf; case _ wf jk =>
+  unfold compile_ctx at cc; simp at cc;
+  rw[Option.bind_eq_some] at cc;
+  cases cc; case _ w cc =>
+  cases cc; case _ cc cc1 =>
+  rw[Option.bind_eq_some] at cc1;
+  cases cc1; case _ w1 cc1 =>
+  cases cc1; case _ cc1 cc2 =>
+  rw[Option.bind_eq_some] at cc2;
+  cases cc2; case _ w2 cc2 =>
+  cases cc2; case _ cc2 cc3 =>
+  cases cc3; cases w1;
+  apply Judgment.wftype;
+  sorry
+  apply @ih w wf cc
+  -- apply compile_preserves_types _ j cc2;
+  -- case _ => apply @ih w wf cc
+  --
+
+case _ => sorry
+case _ => sorry
+
+
+theorem cc_soundness Γ : ⊢s Γ -> (Η : HsCtx Γ) -> compile_ctx Η = .some Γ' -> CompileCtx Γ Γ'
+  := by
+intro wf h j
+induction h using compile_ctx.induct generalizing Γ'
+case _ =>
+  unfold compile_ctx at j; cases j;
+  constructor;
+case _ Γ Η ih =>
+  unfold compile_ctx at j; simp at j;
+  rw[Option.bind_eq_some] at j;
+  cases j; case _ w j =>
+  cases j; case _ j j1 =>
+  rw[Option.bind_eq_some] at j1;
+  cases j1; case _ w1 j1 =>
+  cases j1; case _ j1 e =>
+  cases e; cases wf; case _ wf =>
+  apply CompileCtx.empty;
+  assumption
+  apply compile_preserves_wf Γ wf Η j
+  apply ih wf j
+case _ Γ k Η jk ih =>
+  unfold compile_ctx at j; simp at j;
+  rw[Option.bind_eq_some] at j;
+  cases j; case _ w j =>
+  cases j; case _ j j1 =>
+  rw[Option.bind_eq_some] at j1;
+  cases j1; case _ w1 j1 =>
+  cases j1; case _ j1 j2 =>
+  rw[Option.bind_eq_some] at j2;
+  cases j2; case _ w2 j2 =>
+  cases j2; case _ j2 e =>
+  cases e; cases wf; case _ wf jk' =>
+  apply CompileCtx.kind;
+  assumption
+  apply compile_preserves_wf Γ wf Η j
+  apply ih wf j
+  assumption
+case _ Γ k Η jk ih =>
+  unfold compile_ctx at j; simp at j;
+  rw[Option.bind_eq_some] at j;
+  cases j; case _ w j =>
+  cases j; case _ j j1 =>
+  rw[Option.bind_eq_some] at j1;
+  cases j1; case _ w1 j1 =>
+  cases j1; case _ j1 j2 =>
+  rw[Option.bind_eq_some] at j2;
+  cases j2; case _ w2 j2 =>
+  cases j2; case _ j2 e =>
+  cases e; cases wf; case _ wf jk' =>
+  apply CompileCtx.datatype;
+  assumption
+  apply compile_preserves_wf Γ wf Η j
+  apply ih wf j
+  assumption
+case _  Γ k Η _ ih =>
+  unfold compile_ctx at j; simp at j;
+  rw[Option.bind_eq_some] at j;
+  cases j; case _ w j =>
+  cases j; case _ j j1 =>
+  rw[Option.bind_eq_some] at j1;
+  cases j1; case _ w1 j1 =>
+  cases j1; case _ j1 j2 =>
+  rw[Option.bind_eq_some] at j2;
+  cases j2; case _ w2 j2 =>
+  cases j2; case _ j2 e =>
+  cases e; cases wf; case _ wf jk' =>
+  apply CompileCtx.type;
+  assumption
+  apply compile_preserves_wf Γ wf Η j
+  apply ih wf j
+  assumption
+case _  Γ k Η _ ih =>
+  unfold compile_ctx at j; simp at j;
+  rw[Option.bind_eq_some] at j;
+  cases j; case _ w j =>
+  cases j; case _ j j1 =>
+  rw[Option.bind_eq_some] at j1;
+  cases j1; case _ w1 j1 =>
+  cases j1; case _ j1 j2 =>
+  rw[Option.bind_eq_some] at j2;
+  cases j2; case _ w2 j2 =>
+  cases j2; case _ j2 e =>
+  cases e; cases wf; case _ wf _ vh =>
+  apply CompileCtx.ctor;
+  assumption
+  apply compile_preserves_wf Γ wf Η j
+  apply ih wf j
+  assumption
+case _  Γ k Η _ ih =>
+  unfold compile_ctx at j; simp at j;
+  rw[Option.bind_eq_some] at j;
+  cases j; case _ w j =>
+  cases j; case _ j j1 =>
+  rw[Option.bind_eq_some] at j1;
+  cases j1; case _ w1 j1 =>
+  cases j1; case _ j1 j2 =>
+  rw[Option.bind_eq_some] at j2;
+  cases j2; case _ w2 j2 =>
+  cases j2; case _ j2 e =>
+  cases e; cases wf; case _ wf jk =>
+  apply CompileCtx.openm;
+  assumption
+  apply compile_preserves_wf Γ wf Η j
+  apply ih wf j
+  assumption
+
+-- theorem cc_completeness Γ : ⊢s Γ -> (Η : HsCtx Γ) -> CompileCtx Γ Γ' -> compile_ctx Η = .some Γ'
+--   := by
+-- intro wf h cc
+-- induction cc;
+-- case _ =>
+--   cases h; unfold compile_ctx; rfl;
+-- case _ =>
+--   cases h; cases wf; case _ Γ Γ' _ wf' cc ih h wf =>
+--   unfold compile_ctx; simp
+--   rw[Option.bind_eq_some];
+--   exists Γ'; apply And.intro;
+--   apply ih wf
+--   rw[Option.bind_eq_some];
+--   exists (); apply And.intro;
+--   sorry
+--   simp
 -- case _ => sorry
 -- case _ => sorry
-theorem compile_ctx_type : ∀ Γ Γ',
-  ⊢ Γ' ->
-  CompileCtx Γ Γ' ->
-  (Γ d@ x).get_type = .some τ ->
-  (j : Γ ⊢τ `#x : τ) ->
-  compile_type Γ `#x τ j = .some τ' ->
-  (Γ' @ x).get_type = .some τ' :=
-by
-intro Γ Γ' wf cc gt j c;
-induction cc <;> simp at *;
-case _ => cases gt
-case _ ih1 =>
-  induction x;
-  case _ => simp at *; cases j; case _ j => cases j;
-  case _ ih2 => simp; sorry
-case _ => sorry
-case _ => sorry
-case _ => sorry
--- unfold compile_type at c; cases j; cases c;
+-- case _ => sorry
+-- case _ => sorry
 
 theorem compile_preserves_term_indices :
   ⊢ Γ' ->
