Hs/Metatheory/Uniqueness.lean
@@ -51,7 +51,7 @@ theorem kinds_have_unique_judgments :
 intro h j1 j2;
 apply kinds_have_unique_judgments_lemma h j2 j1 j2;
 
-theorem kinds_compiling_uniqueness :
+theorem compile_kind_uniqueness :
   (∀ Γ (h1 h2 : ⊢s Γ), h1 = h2) ->
   (j1 : Γ ⊢κ t : τ) ->
   (j2 : Γ ⊢κ t : τ) ->
@@ -62,6 +62,21 @@ intro h j1 j2 c1 c2
 have lem := kinds_have_unique_judgments h j1 j2; cases lem;
 rw[c1] at c2; injection c2
 
+@[simp]
+abbrev WellSortedKindInversion : (v : HsVariant) -> Ctx HsTerm -> HsJudgmentArgs v -> Prop
+| .kind => λ Γ => λ (t, τ) => Γ ⊢κ t : τ -> τ = `□
+| _ => λ _ => λ _ => true
+
+theorem well_sorted_kind_inversion_lemma :
+  HsJudgment v Γ idx -> WellSortedKindInversion v Γ idx := by
+intro j;
+induction j <;> simp at *;
+
+theorem well_sorted_kind_inversion :
+  Γ ⊢κ t : τ -> τ = `□ := by
+intro j;
+have lem := well_sorted_kind_inversion_lemma j;
+apply lem j;
 ------------------------------------
 -- Judgments For Types
 ------------------------------------
@@ -71,16 +86,16 @@ theorem types_have_unique_kinds :
   Γ ⊢τ t : k' ->
   k = k' := by
 intro j1 j2;
-induction t generalizing Γ k k';
+induction t generalizing k k'
 all_goals (cases j1)
 case _ =>
   cases j2
   case _ h2 _ _ h1 =>
   rw [<-h1] at h2; injection h2;
 all_goals(cases j2)
-case _ ih1 ih2 A j1 j2 A' j1' j2' =>
-  have u := @ih2 Γ A A' j1 j1'; subst u;
-  have u := @ih1 Γ (A `-k> k) (A `-k> k') j2 j2';
+case _ f a ih1 ih2 k'' hk1 ht1 hk2 ht2 B hk3 ht3 hk4 ht4 =>
+  have u := @ih2 k'' B ht1 ht3; subst u;
+  have u := @ih1 (k'' `-k> k) (k'' `-k> k') ht2 ht4;
   simp at u; apply u;
 case _ => rfl
 case _ => rfl
@@ -119,15 +134,18 @@ case _ Γ _ _ ja _ jb ih1 ih2 =>
   have lem := types_have_unique_kinds ja ja1; cases lem;
   have lem := ih1 ja1 ja2; cases lem
   have lem := ih2 jb1 jb2; cases lem; simp
-case _ Γ _ _ _ _ jf ja ih1 ih2  =>
+case _ Γ _ _ _ _ jf ja jka jkb ih1 ih2 _ _ =>
   intro j1 j2;
   cases j1; cases j2;
   simp at *;
-  case _ ja1 jf1 _ ja2 jf2 =>
+  case _ _ jka1 ja1 jkb1 jf1 _ jka2 ja2 jkb2 jf2 =>
   have lem := types_have_unique_kinds ja1 ja2; cases lem; simp at *;
   have lem := types_have_unique_kinds ja ja1; cases lem;
   have lem := ih1 jf1 jf2; cases lem
-  have lem := ih2 ja1 ja2; cases lem; simp
+  have lem := ih2 ja1 ja2; cases lem; simp;
+  have lem := kinds_have_unique_judgments h jkb1 jkb2; cases lem;
+  have lem := kinds_have_unique_judgments h jka1 jka2; cases lem;
+  simp
 case _ Γ _ _ _ _ _ _ =>
   intro j1 j2;
   cases j1; cases j2;
