Hs/Example.lean
@@ -16,11 +16,27 @@ def idTypeKinding : [] ⊢τ idHsType : `★ := by
     apply HsJudgment.varTy; apply HsJudgment.wfkind; apply HsJudgment.ax (HsJudgment.wfnil);
       apply HsJudgment.wfnil; simp; unfold Frame.is_datatype; unfold Frame.apply; simp;
       unfold Frame.is_kind; simp; unfold Frame.get_type; unfold dnth; unfold Frame.apply; simp;
+      {
+      apply HsJudgment.ax
+      apply HsJudgment.wfkind
+      · apply HsJudgment.ax
+        apply HsJudgment.wfnil
+      · apply HsJudgment.wfnil }
+
     apply HsJudgment.varTy;
       apply HsJudgment.wfempty; apply HsJudgment.wfkind; apply HsJudgment.ax (HsJudgment.wfnil);
       apply HsJudgment.wfnil;
       simp; unfold Frame.is_kind; unfold Frame.apply; simp; unfold Frame.get_type; unfold dnth;
-      unfold dnth; unfold Frame.apply; simp
+      unfold dnth; unfold Frame.apply; simp;
+      {
+        apply HsJudgment.ax
+        apply HsJudgment.wfempty
+        apply HsJudgment.wfkind
+        · apply HsJudgment.ax
+          apply HsJudgment.wfnil
+        · apply HsJudgment.wfnil
+      }
+
 
 def idTyping : [] ⊢t idHsTerm : idHsType := by
  unfold idHsTerm; unfold idHsType;
@@ -29,11 +45,20 @@ def idTyping : [] ⊢t idHsTerm : idHsType := by
    apply HsJudgment.varTy; apply HsJudgment.wfkind; apply HsJudgment.ax (HsJudgment.wfnil);
    apply HsJudgment.wfnil; unfold Frame.is_kind; unfold dnth; unfold Frame.apply; simp;
    unfold Frame.get_type; unfold dnth; unfold Frame.apply; simp;
+   {
+        apply HsJudgment.ax
+        apply HsJudgment.wfkind
+        · apply HsJudgment.ax
+          apply HsJudgment.wfnil
+        · apply HsJudgment.wfnil
+   };
+
    apply HsJudgment.var;
    apply HsJudgment.wftype; apply HsJudgment.varTy;
    apply HsJudgment.wfkind; apply HsJudgment.ax (HsJudgment.wfnil); apply HsJudgment.wfnil;
    unfold Frame.is_kind; unfold dnth; unfold Frame.apply; simp;
    unfold Frame.get_type; unfold dnth; unfold Frame.apply; simp;
+   apply HsJudgment.ax; apply HsJudgment.wfkind; apply HsJudgment.ax (HsJudgment.wfnil); apply HsJudgment.wfnil;
    apply HsJudgment.wfkind; apply HsJudgment.ax (HsJudgment.wfnil);
    apply HsJudgment.wfnil; unfold Frame.is_type; unfold dnth; unfold Frame.apply; simp;
    unfold Frame.get_type; unfold dnth; unfold Frame.apply; simp;
@@ -42,22 +67,52 @@ def idTyping : [] ⊢t idHsTerm : idHsType := by
      apply HsJudgment.wfkind; apply HsJudgment.ax (HsJudgment.wfnil); apply HsJudgment.wfnil;
      unfold Frame.is_kind; unfold dnth; unfold Frame.apply; simp;
      unfold Frame.get_type; unfold dnth; unfold Frame.apply; simp;
+     {
+  apply HsJudgment.ax
+  apply HsJudgment.wfkind
+  · apply HsJudgment.ax
+    apply HsJudgment.wfnil
+  · apply HsJudgment.wfnil
+     };
      apply HsJudgment.varTy;
      apply HsJudgment.wfempty;
      apply HsJudgment.wfkind; apply HsJudgment.ax (HsJudgment.wfnil); apply HsJudgment.wfnil;
    unfold Frame.is_kind; unfold dnth; unfold Frame.apply; simp; unfold Frame.apply; simp;
    unfold Frame.get_type; unfold dnth; unfold Frame.apply; unfold dnth; simp; unfold Frame.apply; simp;
+   {
+  apply HsJudgment.ax
+  apply HsJudgment.wfempty
+  apply HsJudgment.wfkind
+  · apply HsJudgment.ax
+    apply HsJudgment.wfnil
+  · apply HsJudgment.wfnil
+  };
    apply HsJudgment.ax (HsJudgment.wfnil);
    apply HsJudgment.arrow;
    apply HsJudgment.varTy;
       apply HsJudgment.wfkind; apply HsJudgment.ax (HsJudgment.wfnil); apply HsJudgment.wfnil;
       unfold Frame.is_kind; unfold dnth; unfold Frame.apply; simp;
       unfold Frame.get_type; unfold dnth; unfold Frame.apply; simp;
+   {
+  apply HsJudgment.ax
+  apply HsJudgment.wfkind
+  · apply HsJudgment.ax
+    apply HsJudgment.wfnil
+  · apply HsJudgment.wfnil
+  };
    apply HsJudgment.varTy;
       apply HsJudgment.wfempty; apply HsJudgment.wfkind; apply HsJudgment.ax (HsJudgment.wfnil);
       apply HsJudgment.wfnil;
       unfold Frame.is_kind; unfold dnth; unfold Frame.apply; simp; unfold Frame.apply; simp;
       unfold Frame.get_type; unfold dnth; unfold Frame.apply; simp; unfold Frame.apply; simp;
+      {
+  apply HsJudgment.ax
+  apply HsJudgment.wfempty
+  apply HsJudgment.wfkind
+  · apply HsJudgment.ax
+    apply HsJudgment.wfnil
+  · apply HsJudgment.wfnil
+      }
 
 def idType := compile_type [] idHsType `★ idTypeKinding
 def idTerm := compile_term [] idHsTerm idHsType idTyping
@@ -70,588 +125,706 @@ def idTerm := compile_term [] idHsTerm idHsType idTyping
 #eval idTerm
 
 def MbCtx : Ctx HsTerm :=
-  [ .ctor (`∀{`★} `#2 `•k `#0)   -- Nothing :: ∀ a. Maybe a
-  , .ctor (`∀{`★} `#0 → `#2 `•k `#1)          -- Just :: ∀ a. a -> Maybe a
+  [ .ctor (`∀{`★} `#2 `•k `#0)          -- Nothing :: ∀ a. Maybe a
+  , .ctor (`∀{`★} `#0 → `#2 `•k `#1)    -- Just :: ∀ a. a -> Maybe a
   , .datatype (`★ `-k> `★) ]
 
 -- set_option trace.aesop.tree true
 -- set_option trace.aesop true
-def MaybeCtx : HsCtx MbCtx :=
-  .ctor
-    (.ctor
-      (.datatype .nil ⟨`★ `-k> `★ ,
-        by apply HsJudgment.arrowk; apply HsJudgment.ax; apply HsJudgment.wfnil
-           apply HsJudgment.ax; apply HsJudgment.wfnil⟩)
-      ⟨`∀{`★} `#0 → `#2 `•k `#1,
-        by apply HsJudgment.allt
-           apply HsJudgment.ax
-           apply HsJudgment.wfdatatype
-           apply HsJudgment.arrowk
-           apply HsJudgment.ax
-           apply HsJudgment.wfnil
-           apply HsJudgment.ax
-           apply HsJudgment.wfnil
-           apply HsJudgment.wfnil
-           apply HsJudgment.arrow
-           apply HsJudgment.varTy
-           apply HsJudgment.wfkind
-           apply HsJudgment.ax
-           apply HsJudgment.wfdatatype
-           apply HsJudgment.arrowk
-           apply HsJudgment.ax
-           apply HsJudgment.wfnil
-           apply HsJudgment.ax
-           apply HsJudgment.wfnil
-           apply HsJudgment.wfnil
-           apply HsJudgment.wfdatatype
-           apply HsJudgment.arrowk
-           apply HsJudgment.ax
-           apply HsJudgment.wfnil
-           apply HsJudgment.ax
-           apply HsJudgment.wfnil
-           apply HsJudgment.wfnil
-           simp_all only [dnth, substType_HsTerm, Bool.or_eq_true]
-           apply Or.inr; rfl
-           simp_all only [dnth, substType_HsTerm, Frame.get_type_apply_commute]; rfl
-           apply HsJudgment.appk
-           apply HsJudgment.varTy
-           apply HsJudgment.wfempty
-           apply HsJudgment.wfkind
-           apply HsJudgment.ax
-           apply HsJudgment.wfdatatype
-           apply HsJudgment.arrowk
-           apply HsJudgment.ax
-           apply HsJudgment.wfnil
-           apply HsJudgment.ax
-           apply HsJudgment.wfnil
-           apply HsJudgment.wfnil
-           apply HsJudgment.wfdatatype
-           apply HsJudgment.arrowk;
-             apply HsJudgment.ax; apply HsJudgment.wfnil;
-             apply HsJudgment.ax; apply HsJudgment.wfnil;
-           apply HsJudgment.wfnil
-           simp_all only [dnth, substType_HsTerm, Bool.or_eq_true, Frame.apply_compose, Frame.apply]
-           simp; apply Or.inl; unfold Frame.is_datatype; simp
-           unfold Frame.get_type; unfold dnth; unfold dnth; simp;
-           simp_all only[Frame.apply_compose, Frame.apply]; simp; rfl;
-           apply HsJudgment.varTy
-           apply HsJudgment.wfempty
-           apply HsJudgment.wfkind
-           apply HsJudgment.ax
-           apply HsJudgment.wfdatatype
-           apply HsJudgment.arrowk
-           apply HsJudgment.ax
-           apply HsJudgment.wfnil
-           apply HsJudgment.ax
-           apply HsJudgment.wfnil
-           apply HsJudgment.wfnil
-           apply HsJudgment.wfdatatype
-           apply HsJudgment.arrowk
-           apply HsJudgment.ax
-           apply HsJudgment.wfnil
-           apply HsJudgment.ax
-           apply HsJudgment.wfnil
-           apply HsJudgment.wfnil
-           simp_all only [dnth, substType_HsTerm, Bool.or_eq_true]
-           apply Or.inr; rfl
-           simp_all only [dnth, substType_HsTerm, Frame.get_type_apply_commute, Option.map_map]; rfl
-      ⟩)
-    ⟨`∀{`★} `#2 `•k `#0, by
-      apply HsJudgment.allt
-      apply HsJudgment.ax;
-        apply HsJudgment.wfctor;
-        { apply HsJudgment.allt;
-          apply HsJudgment.ax
-          apply HsJudgment.wfdatatype
-          apply HsJudgment.arrowk
-          apply HsJudgment.ax
-          apply HsJudgment.wfnil
-          apply HsJudgment.ax
-          apply HsJudgment.wfnil
-          apply HsJudgment.wfnil
-          apply HsJudgment.arrow
-          apply HsJudgment.varTy
-          apply HsJudgment.wfkind
-          apply HsJudgment.ax
-          apply HsJudgment.wfdatatype
-          apply HsJudgment.arrowk
-          apply HsJudgment.ax
-          apply HsJudgment.wfnil
-          apply HsJudgment.ax
-          apply HsJudgment.wfnil
-          apply HsJudgment.wfnil
-          apply HsJudgment.wfdatatype
-          apply HsJudgment.arrowk
-          apply HsJudgment.ax
-          apply HsJudgment.wfnil
-          apply HsJudgment.ax
-          apply HsJudgment.wfnil
-          apply HsJudgment.wfnil
-          simp_all only [dnth, substType_HsTerm, Bool.or_eq_true]
-          apply Or.inr; rfl;
-          simp_all only [dnth, substType_HsTerm, Frame.get_type_apply_commute]; rfl;
-          apply HsJudgment.appk
+-- def MaybeCtx : HsCtx MbCtx :=
+--   .ctor
+--     (.ctor
+--       (.datatype .nil ⟨`★ `-k> `★ ,
+--         by apply HsJudgment.arrowk; apply HsJudgment.ax; apply HsJudgment.wfnil
+--            apply HsJudgment.ax; apply HsJudgment.wfnil⟩)
+--       ⟨`∀{`★} `#0 → `#2 `•k `#1,
+--         by apply HsJudgment.allt
+--            apply HsJudgment.ax
+--            apply HsJudgment.wfdatatype
+--            apply HsJudgment.arrowk
+--            apply HsJudgment.ax
+--            apply HsJudgment.wfnil
+--            apply HsJudgment.ax
+--            apply HsJudgment.wfnil
+--            apply HsJudgment.wfnil
+--            apply HsJudgment.arrow
+--            apply HsJudgment.varTy
+--            apply HsJudgment.wfkind
+--            apply HsJudgment.ax
+--            apply HsJudgment.wfdatatype
+--            apply HsJudgment.arrowk
+--            apply HsJudgment.ax
+--            apply HsJudgment.wfnil
+--            apply HsJudgment.ax
+--            apply HsJudgment.wfnil
+--            apply HsJudgment.wfnil
+--            apply HsJudgment.wfdatatype
+--            apply HsJudgment.arrowk
+--            apply HsJudgment.ax
+--            apply HsJudgment.wfnil
+--            apply HsJudgment.ax
+--            apply HsJudgment.wfnil
+--            apply HsJudgment.wfnil
+--            simp_all only [dnth, substType_HsTerm, Bool.or_eq_true]
+--            apply Or.inr; rfl
+--            simp_all only [dnth, substType_HsTerm, Frame.get_type_apply_commute]; rfl
+--            apply HsJudgment.appk
+--            apply HsJudgment.varTy
+--            apply HsJudgment.wfempty
+--            apply HsJudgment.wfkind
+--            apply HsJudgment.ax
+--            apply HsJudgment.wfdatatype
+--            apply HsJudgment.arrowk
+--            apply HsJudgment.ax
+--            apply HsJudgment.wfnil
+--            apply HsJudgment.ax
+--            apply HsJudgment.wfnil
+--            apply HsJudgment.wfnil
+--            apply HsJudgment.wfdatatype
+--            apply HsJudgment.arrowk;
+--              apply HsJudgment.ax; apply HsJudgment.wfnil;
+--              apply HsJudgment.ax; apply HsJudgment.wfnil;
+--            apply HsJudgment.wfnil
+--            simp_all only [dnth, substType_HsTerm, Bool.or_eq_true, Frame.apply_compose, Frame.apply]
+--            simp; apply Or.inl; unfold Frame.is_datatype; simp
+--            unfold Frame.get_type; unfold dnth; unfold dnth; simp;
+--            simp_all only[Frame.apply_compose, Frame.apply]; simp; rfl;
+--            apply HsJudgment.varTy
+--            apply HsJudgment.wfempty
+--            apply HsJudgment.wfkind
+--            apply HsJudgment.ax
+--            apply HsJudgment.wfdatatype
+--            apply HsJudgment.arrowk
+--            apply HsJudgment.ax
+--            apply HsJudgment.wfnil
+--            apply HsJudgment.ax
+--            apply HsJudgment.wfnil
+--            apply HsJudgment.wfnil
+--            apply HsJudgment.wfdatatype
+--            apply HsJudgment.arrowk
+--            apply HsJudgment.ax
+--            apply HsJudgment.wfnil
+--            apply HsJudgment.ax
+--            apply HsJudgment.wfnil
+--            apply HsJudgment.wfnil
+--            simp_all only [dnth, substType_HsTerm, Bool.or_eq_true]
+--            apply Or.inr; rfl
+--            simp_all only [dnth, substType_HsTerm, Frame.get_type_apply_commute, Option.map_map]; rfl
+--            {
+--                 apply HsJudgment.ax
+--                 apply HsJudgment.wfempty
+--                 apply HsJudgment.wfkind
+--                 · apply HsJudgment.ax
+--                   apply HsJudgment.wfdatatype
+--                   · apply HsJudgment.arrowk
+--                     · apply HsJudgment.ax
+--                       apply HsJudgment.wfnil
+--                     · apply HsJudgment.ax
+--                       apply HsJudgment.wfnil
+--                   · apply HsJudgment.wfnil
+--                 · apply HsJudgment.wfdatatype
+--                   · apply HsJudgment.arrowk
+--                     · apply HsJudgment.ax
+--                       apply HsJudgment.wfnil
+--                     · apply HsJudgment.ax
+--                       apply HsJudgment.wfnil
+--                   · apply HsJudgment.wfnil
+--            }
+--            {
+--                 apply HsJudgment.ax
+--                 apply HsJudgment.wfempty
+--                 apply HsJudgment.wfkind
+--                 · apply HsJudgment.ax
+--                   apply HsJudgment.wfdatatype
+--                   · apply HsJudgment.arrowk
+--                     · apply HsJudgment.ax
+--                       apply HsJudgment.wfnil
+--                     · apply HsJudgment.ax
+--                       apply HsJudgment.wfnil
+--                   · apply HsJudgment.wfnil
+--                 · apply HsJudgment.wfdatatype
+--                   · apply HsJudgment.arrowk
+--                     · apply HsJudgment.ax
+--                       apply HsJudgment.wfnil
+--                     · apply HsJudgment.ax
+--                       apply HsJudgment.wfnil
+--                   · apply HsJudgment.wfnil
+--            }
+--       ⟩)
+--     ⟨`∀{`★} `#2 `•k `#0, by
+--       apply HsJudgment.allt
+--       apply HsJudgment.ax;
+--         apply HsJudgment.wfctor;
+--         { apply HsJudgment.allt;
+--           apply HsJudgment.ax
+--           apply HsJudgment.wfdatatype
+--           apply HsJudgment.arrowk
+--           apply HsJudgment.ax
+--           apply HsJudgment.wfnil
+--           apply HsJudgment.ax
+--           apply HsJudgment.wfnil
+--           apply HsJudgment.wfnil
+--           apply HsJudgment.arrow
+--           apply HsJudgment.varTy
+--           apply HsJudgment.wfkind
+--           apply HsJudgment.ax
+--           apply HsJudgment.wfdatatype
+--           apply HsJudgment.arrowk
+--           apply HsJudgment.ax
+--           apply HsJudgment.wfnil
+--           apply HsJudgment.ax
+--           apply HsJudgment.wfnil
+--           apply HsJudgment.wfnil
+--           apply HsJudgment.wfdatatype
+--           apply HsJudgment.arrowk
+--           apply HsJudgment.ax
+--           apply HsJudgment.wfnil
+--           apply HsJudgment.ax
+--           apply HsJudgment.wfnil
+--           apply HsJudgment.wfnil
+--           simp_all only [dnth, substType_HsTerm, Bool.or_eq_true]
+--           apply Or.inr; rfl;
+--           simp_all only [dnth, substType_HsTerm, Frame.get_type_apply_commute]; rfl;
+--           apply HsJudgment.appk
+--           apply HsJudgment.varTy
+--           apply HsJudgment.wfempty
+--           apply HsJudgment.wfkind
+--           apply HsJudgment.ax
+--           apply HsJudgment.wfdatatype
+--           apply HsJudgment.arrowk
+--           apply HsJudgment.ax
+--           apply HsJudgment.wfnil
+--           apply HsJudgment.ax
+--           apply HsJudgment.wfnil
+--           apply HsJudgment.wfnil
+--           apply HsJudgment.wfdatatype
+--           apply HsJudgment.arrowk
+--           apply HsJudgment.ax
+--           apply HsJudgment.wfnil
+--           apply HsJudgment.ax
+--           apply HsJudgment.wfnil
+--           apply HsJudgment.wfnil
+--           simp_all only [dnth, substType_HsTerm, Bool.or_eq_true]
+--           apply Or.inl; rfl
+--           simp_all only [dnth, substType_HsTerm, Frame.get_type_apply_commute, Option.map_map]; rfl;
 
-          apply HsJudgment.varTy
-          apply HsJudgment.wfempty
-          apply HsJudgment.wfkind
-          apply HsJudgment.ax
-          apply HsJudgment.wfdatatype
-          apply HsJudgment.arrowk
-          apply HsJudgment.ax
-          apply HsJudgment.wfnil
-          apply HsJudgment.ax
-          apply HsJudgment.wfnil
-          apply HsJudgment.wfnil
-          apply HsJudgment.wfdatatype
-          apply HsJudgment.arrowk
-          apply HsJudgment.ax
-          apply HsJudgment.wfnil
-          apply HsJudgment.ax
-          apply HsJudgment.wfnil
-          apply HsJudgment.wfnil
-          simp_all only [dnth, substType_HsTerm, Bool.or_eq_true]
-          apply Or.inl; rfl
-          simp_all only [dnth, substType_HsTerm, Frame.get_type_apply_commute, Option.map_map]; rfl;
+--           -- simp_all only [Function.comp_apply, HsTerm.subst_const]
+--           apply HsJudgment.varTy
+--           apply HsJudgment.wfempty
+--           apply HsJudgment.wfkind
+--           apply HsJudgment.ax
+--           apply HsJudgment.wfdatatype
+--           apply HsJudgment.arrowk
+--           apply HsJudgment.ax
+--           apply HsJudgment.wfnil
+--           apply HsJudgment.ax
+--           apply HsJudgment.wfnil
+--           apply HsJudgment.wfnil
+--           apply HsJudgment.wfdatatype
+--           apply HsJudgment.arrowk
+--           apply HsJudgment.ax
+--           apply HsJudgment.wfnil
+--           apply HsJudgment.ax
+--           apply HsJudgment.wfnil
+--           apply HsJudgment.wfnil
+--           simp_all only [dnth, substType_HsTerm, Bool.or_eq_true, Frame.apply, Frame.is_kind]
+--           apply Or.inr; simp;
+--           simp_all only [dnth, Frame.get_type_apply_commute, Option.map_map, Frame.get_type];
+--           unfold Frame.apply; simp;
+--           {
+--                 simp_all only [HsTerm.smap, HsTerm.smap.eq_3]
+--                 apply HsJudgment.ax
+--                 apply HsJudgment.wfempty
+--                 apply HsJudgment.wfkind
+--                 · apply HsJudgment.ax
+--                   apply HsJudgment.wfdatatype
+--                   · apply HsJudgment.arrowk
+--                     · apply HsJudgment.ax
+--                       apply HsJudgment.wfnil
+--                     · apply HsJudgment.ax
+--                       apply HsJudgment.wfnil
+--                   · apply HsJudgment.wfnil
+--                 · apply HsJudgment.wfdatatype
+--                   · apply HsJudgment.arrowk
+--                     · apply HsJudgment.ax
+--                       apply HsJudgment.wfnil
+--                     · apply HsJudgment.ax
+--                       apply HsJudgment.wfnil
+--                   · apply HsJudgment.wfnil
+--           };
+--           {
+--                 apply HsJudgment.ax
+--                 apply HsJudgment.wfempty
+--                 apply HsJudgment.wfkind
+--                 · apply HsJudgment.ax
+--                   apply HsJudgment.wfdatatype
+--                   · apply HsJudgment.arrowk
+--                     · apply HsJudgment.ax
+--                       apply HsJudgment.wfnil
+--                     · apply HsJudgment.ax
+--                       apply HsJudgment.wfnil
+--                   · apply HsJudgment.wfnil
+--                 · apply HsJudgment.wfdatatype
+--                   · apply HsJudgment.arrowk
+--                     · apply HsJudgment.ax
+--                       apply HsJudgment.wfnil
+--                     · apply HsJudgment.ax
+--                       apply HsJudgment.wfnil
+--                   · apply HsJudgment.wfnil
+--           }};
+--         apply HsJudgment.wfdatatype;   apply HsJudgment.arrowk; apply HsJudgment.ax;
+--         apply HsJudgment.wfnil; apply HsJudgment.ax; apply HsJudgment.wfnil; apply HsJudgment.wfnil;
+--         apply ValidHsCtorType.all; apply ValidHsCtorType.arrow; apply ValidHsCtorType.refl;
+--         unfold HsValidHeadVariable; simp; rfl
+--       apply HsJudgment.appk;
+--         apply HsJudgment.varTy;
+--           apply HsJudgment.wfkind;
+--             apply HsJudgment.ax;
+--             {
+--               apply HsJudgment.wfctor;
+--               {
+--                 apply HsJudgment.allt
+--                 · apply HsJudgment.ax
+--                   apply HsJudgment.wfdatatype
+--                   · apply HsJudgment.arrowk
+--                     · apply HsJudgment.ax
+--                       apply HsJudgment.wfnil
+--                     · apply HsJudgment.ax
+--                       apply HsJudgment.wfnil
+--                   · apply HsJudgment.wfnil
+--                 · apply HsJudgment.arrow
+--                   · apply HsJudgment.varTy
+--                     · apply HsJudgment.wfkind
+--                       · apply HsJudgment.ax
+--                         apply HsJudgment.wfdatatype
+--                         · apply HsJudgment.arrowk
+--                           · apply HsJudgment.ax
+--                             apply HsJudgment.wfnil
+--                           · apply HsJudgment.ax
+--                             apply HsJudgment.wfnil
+--                         · apply HsJudgment.wfnil
+--                       · apply HsJudgment.wfdatatype
+--                         · apply HsJudgment.arrowk
+--                           · apply HsJudgment.ax
+--                             apply HsJudgment.wfnil
+--                           · apply HsJudgment.ax
+--                             apply HsJudgment.wfnil
+--                         · apply HsJudgment.wfnil
+--                     · simp_all only [dnth, substType_HsTerm, Bool.or_eq_true]
+--                       apply Or.inr
+--                       rfl
+--                     · simp_all only [dnth, substType_HsTerm, Frame.get_type_apply_commute]
+--                       rfl
+--                   · apply HsJudgment.appk
+--                     on_goal 2 => {
+--                       apply HsJudgment.varTy
+--                       · apply HsJudgment.wfempty
+--                         apply HsJudgment.wfkind
+--                         · apply HsJudgment.ax
+--                           apply HsJudgment.wfdatatype
+--                           · apply HsJudgment.arrowk
+--                             · apply HsJudgment.ax
+--                               apply HsJudgment.wfnil
+--                             · apply HsJudgment.ax
+--                               apply HsJudgment.wfnil
+--                           · apply HsJudgment.wfnil
+--                         · apply HsJudgment.wfdatatype
+--                           · apply HsJudgment.arrowk
+--                             · apply HsJudgment.ax
+--                               apply HsJudgment.wfnil
+--                             · apply HsJudgment.ax
+--                               apply HsJudgment.wfnil
+--                           · apply HsJudgment.wfnil
+--                       · simp_all only [dnth, substType_HsTerm, Bool.or_eq_true]
+--                         apply Or.inr
+--                         rfl
+--                       · simp_all only [dnth, substType_HsTerm, Frame.get_type_apply_commute, Option.map_map]
+--                         rfl
+--                     }
+--                     · simp_all only [Function.comp_apply, HsTerm.subst_const]
+--                       apply HsJudgment.varTy
+--                       · apply HsJudgment.wfempty
+--                         apply HsJudgment.wfkind
+--                         · apply HsJudgment.ax
+--                           apply HsJudgment.wfdatatype
+--                           · apply HsJudgment.arrowk
+--                             · apply HsJudgment.ax
+--                               apply HsJudgment.wfnil
+--                             · apply HsJudgment.ax
+--                               apply HsJudgment.wfnil
+--                           · apply HsJudgment.wfnil
+--                         · apply HsJudgment.wfdatatype
+--                           · apply HsJudgment.arrowk
+--                             · apply HsJudgment.ax
+--                               apply HsJudgment.wfnil
+--                             · apply HsJudgment.ax
+--                               apply HsJudgment.wfnil
+--                           · apply HsJudgment.wfnil
 
-          -- simp_all only [Function.comp_apply, HsTerm.subst_const]
-          apply HsJudgment.varTy
-          apply HsJudgment.wfempty
-          apply HsJudgment.wfkind
-          apply HsJudgment.ax
-          apply HsJudgment.wfdatatype
-          apply HsJudgment.arrowk
-          apply HsJudgment.ax
-          apply HsJudgment.wfnil
-          apply HsJudgment.ax
-          apply HsJudgment.wfnil
-          apply HsJudgment.wfnil
-          apply HsJudgment.wfdatatype
-          apply HsJudgment.arrowk
-          apply HsJudgment.ax
-          apply HsJudgment.wfnil
-          apply HsJudgment.ax
-          apply HsJudgment.wfnil
-          apply HsJudgment.wfnil
-          simp_all only [dnth, substType_HsTerm, Bool.or_eq_true, Frame.apply, Frame.is_kind]
-          apply Or.inr; simp;
-          simp_all only [dnth, Frame.get_type_apply_commute, Option.map_map, Frame.get_type];
-          unfold Frame.apply; simp};
-        apply HsJudgment.wfdatatype;   apply HsJudgment.arrowk; apply HsJudgment.ax;
-        apply HsJudgment.wfnil; apply HsJudgment.ax; apply HsJudgment.wfnil; apply HsJudgment.wfnil;
-        apply ValidHsCtorType.all; apply ValidHsCtorType.arrow; apply ValidHsCtorType.refl;
-        unfold HsValidHeadVariable; simp; rfl
-      apply HsJudgment.appk;
-        apply HsJudgment.varTy;
-          apply HsJudgment.wfkind;
-            apply HsJudgment.ax;
-            {
-              apply HsJudgment.wfctor;
-              {
-                apply HsJudgment.allt
-                · apply HsJudgment.ax
-                  apply HsJudgment.wfdatatype
-                  · apply HsJudgment.arrowk
-                    · apply HsJudgment.ax
-                      apply HsJudgment.wfnil
-                    · apply HsJudgment.ax
-                      apply HsJudgment.wfnil
-                  · apply HsJudgment.wfnil
-                · apply HsJudgment.arrow
-                  · apply HsJudgment.varTy
-                    · apply HsJudgment.wfkind
-                      · apply HsJudgment.ax
-                        apply HsJudgment.wfdatatype
-                        · apply HsJudgment.arrowk
-                          · apply HsJudgment.ax
-                            apply HsJudgment.wfnil
-                          · apply HsJudgment.ax
-                            apply HsJudgment.wfnil
-                        · apply HsJudgment.wfnil
-                      · apply HsJudgment.wfdatatype
-                        · apply HsJudgment.arrowk
-                          · apply HsJudgment.ax
-                            apply HsJudgment.wfnil
-                          · apply HsJudgment.ax
-                            apply HsJudgment.wfnil
-                        · apply HsJudgment.wfnil
-                    · simp_all only [dnth, substType_HsTerm, Bool.or_eq_true]
-                      apply Or.inr
-                      rfl
-                    · simp_all only [dnth, substType_HsTerm, Frame.get_type_apply_commute]
-                      rfl
-                  · apply HsJudgment.appk
-                    on_goal 2 => {
-                      apply HsJudgment.varTy
-                      · apply HsJudgment.wfempty
-                        apply HsJudgment.wfkind
-                        · apply HsJudgment.ax
-                          apply HsJudgment.wfdatatype
-                          · apply HsJudgment.arrowk
-                            · apply HsJudgment.ax
-                              apply HsJudgment.wfnil
-                            · apply HsJudgment.ax
-                              apply HsJudgment.wfnil
-                          · apply HsJudgment.wfnil
-                        · apply HsJudgment.wfdatatype
-                          · apply HsJudgment.arrowk
-                            · apply HsJudgment.ax
-                              apply HsJudgment.wfnil
-                            · apply HsJudgment.ax
-                              apply HsJudgment.wfnil
-                          · apply HsJudgment.wfnil
-                      · simp_all only [dnth, substType_HsTerm, Bool.or_eq_true]
-                        apply Or.inr
-                        rfl
-                      · simp_all only [dnth, substType_HsTerm, Frame.get_type_apply_commute, Option.map_map]
-                        rfl
-                    }
-                    · simp_all only [Function.comp_apply, HsTerm.subst_const]
-                      apply HsJudgment.varTy
-                      · apply HsJudgment.wfempty
-                        apply HsJudgment.wfkind
-                        · apply HsJudgment.ax
-                          apply HsJudgment.wfdatatype
-                          · apply HsJudgment.arrowk
-                            · apply HsJudgment.ax
-                              apply HsJudgment.wfnil
-                            · apply HsJudgment.ax
-                              apply HsJudgment.wfnil
-                          · apply HsJudgment.wfnil
-                        · apply HsJudgment.wfdatatype
-                          · apply HsJudgment.arrowk
-                            · apply HsJudgment.ax
-                              apply HsJudgment.wfnil
-                            · apply HsJudgment.ax
-                              apply HsJudgment.wfnil
-                          · apply HsJudgment.wfnil
-                      · simp_all only [dnth, substType_HsTerm, Bool.or_eq_true]
-                        apply Or.inl
-                        rfl
-                      · simp_all only [dnth, substType_HsTerm, Frame.get_type_apply_commute, Option.map_map]
-                        rfl
+--                       · simp_all only [dnth, substType_HsTerm, Bool.or_eq_true]; apply Or.inl; rfl
+--                       · simp_all only [dnth, substType_HsTerm, Frame.get_type_apply_commute, Option.map_map]
+--                         rfl
+--               };
+--               {
+--                 apply HsJudgment.wfdatatype
+--                 · apply HsJudgment.arrowk
+--                   · apply HsJudgment.ax
+--                     apply HsJudgment.wfnil
+--                   · apply HsJudgment.ax
+--                     apply HsJudgment.wfnil
+--                 · apply HsJudgment.wfnil
+--               };
+--               {
+--                 apply ValidHsCtorType.all; apply ValidHsCtorType.arrow;
+--                 apply ValidHsCtorType.refl; unfold HsValidHeadVariable; simp;
+--                 simp_all only [Frame.apply, Frame.is_datatype];
+--               };
+--             };
+--             apply HsJudgment.wfctor;
+--             apply HsJudgment.allt;
+--             {
+--                 apply HsJudgment.ax
+--                 apply HsJudgment.wfdatatype
+--                 · apply HsJudgment.arrowk
+--                   · apply HsJudgment.ax
+--                     apply HsJudgment.wfnil
+--                   · apply HsJudgment.ax
+--                     apply HsJudgment.wfnil
+--                 · apply HsJudgment.wfnil
+--             };
+--             {
+--                 apply HsJudgment.arrow
+--                 · apply HsJudgment.varTy
+--                   · apply HsJudgment.wfkind
+--                     · apply HsJudgment.ax
+--                       apply HsJudgment.wfdatatype
+--                       · apply HsJudgment.arrowk
+--                         · apply HsJudgment.ax
+--                           apply HsJudgment.wfnil
+--                         · apply HsJudgment.ax
+--                           apply HsJudgment.wfnil
+--                       · apply HsJudgment.wfnil
+--                     · apply HsJudgment.wfdatatype
+--                       · apply HsJudgment.arrowk
+--                         · apply HsJudgment.ax
+--                           apply HsJudgment.wfnil
+--                         · apply HsJudgment.ax
+--                           apply HsJudgment.wfnil
+--                       · apply HsJudgment.wfnil
+--                   · simp_all only [dnth, substType_HsTerm, Bool.or_eq_true]; apply Or.inr; rfl
+--                   · simp_all only [dnth, substType_HsTerm, Frame.get_type_apply_commute]; rfl
+--                 · apply HsJudgment.appk
+--                   · apply HsJudgment.varTy
+--                     · apply HsJudgment.wfempty
+--                       apply HsJudgment.wfkind
+--                       · apply HsJudgment.ax
+--                         apply HsJudgment.wfdatatype
+--                         · apply HsJudgment.arrowk
+--                           · apply HsJudgment.ax
+--                             apply HsJudgment.wfnil
+--                           · apply HsJudgment.ax
+--                             apply HsJudgment.wfnil
+--                         · apply HsJudgment.wfnil
+--                       · apply HsJudgment.wfdatatype
+--                         · apply HsJudgment.arrowk
+--                           · apply HsJudgment.ax
+--                             apply HsJudgment.wfnil
+--                           · apply HsJudgment.ax
+--                             apply HsJudgment.wfnil
+--                         · apply HsJudgment.wfnil
+--                     · simp_all only [dnth, substType_HsTerm, Bool.or_eq_true]
+--                       apply Or.inl; rfl
+--                     · simp_all only [dnth, substType_HsTerm, Frame.get_type_apply_commute, Option.map_map]; rfl
+--                   · simp_all only [HsTerm.smap, HsTerm.smap.eq_3]
+--                     apply HsJudgment.varTy
+--                     · apply HsJudgment.wfempty
+--                       apply HsJudgment.wfkind
+--                       · apply HsJudgment.ax
+--                         apply HsJudgment.wfdatatype
+--                         · apply HsJudgment.arrowk
+--                           · apply HsJudgment.ax
+--                             apply HsJudgment.wfnil
+--                           · apply HsJudgment.ax
+--                             apply HsJudgment.wfnil
+--                         · apply HsJudgment.wfnil
+--                       · apply HsJudgment.wfdatatype
+--                         · apply HsJudgment.arrowk
+--                           · apply HsJudgment.ax
+--                             apply HsJudgment.wfnil
+--                           · apply HsJudgment.ax
+--                             apply HsJudgment.wfnil
+--                         · apply HsJudgment.wfnil
+--                     · simp_all only [dnth, substType_HsTerm, Bool.or_eq_true]
+--                       apply Or.inr
+--                       rfl
+--                     · simp_all only [dnth, substType_HsTerm, Frame.get_type_apply_commute, Option.map_map]
+--                       rfl
+--                   {
+--                         simp_all only [HsTerm.smap]
+--                         apply HsJudgment.ax
+--                         apply HsJudgment.wfempty
+--                         apply HsJudgment.wfkind
+--                         · apply HsJudgment.ax
+--                           apply HsJudgment.wfdatatype
+--                           · apply HsJudgment.arrowk
+--                             · apply HsJudgment.ax
+--                               apply HsJudgment.wfnil
+--                             · apply HsJudgment.ax
+--                               apply HsJudgment.wfnil
+--                           · apply HsJudgment.wfnil
+--                         · apply HsJudgment.wfdatatype
+--                           · apply HsJudgment.arrowk
+--                             · apply HsJudgment.ax
+--                               apply HsJudgment.wfnil
+--                             · apply HsJudgment.ax
+--                               apply HsJudgment.wfnil
+--                           · apply HsJudgment.wfnil
+--                   }
+--                   {
+--                         apply HsJudgment.ax
+--                         apply HsJudgment.wfempty
+--                         apply HsJudgment.wfkind
+--                         · apply HsJudgment.ax
+--                           apply HsJudgment.wfdatatype
+--                           · apply HsJudgment.arrowk
+--                             · apply HsJudgment.ax
+--                               apply HsJudgment.wfnil
+--                             · apply HsJudgment.ax
+--                               apply HsJudgment.wfnil
+--                           · apply HsJudgment.wfnil
+--                         · apply HsJudgment.wfdatatype
+--                           · apply HsJudgment.arrowk
+--                             · apply HsJudgment.ax
+--                               apply HsJudgment.wfnil
+--                             · apply HsJudgment.ax
+--                               apply HsJudgment.wfnil
+--                           · apply HsJudgment.wfnil
+--                   }
+--             };
+--             apply HsJudgment.wfdatatype;
+--             apply HsJudgment.arrowk;
+--             apply HsJudgment.ax; apply HsJudgment.wfnil;
+--             apply HsJudgment.ax; apply HsJudgment.wfnil;
+--             apply HsJudgment.wfnil;
+--             apply ValidHsCtorType.all; apply ValidHsCtorType.arrow;
+--             apply ValidHsCtorType.refl; unfold HsValidHeadVariable; simp;
+--             simp_all only [Frame.apply, Frame.is_datatype];
+--           simp; apply Or.inl; rfl;
+--           unfold Frame.get_type; unfold dnth; unfold Frame.apply; unfold dnth;
+--           simp; unfold Frame.apply; simp; rfl;
+--         apply HsJudgment.varTy;
+--           {apply HsJudgment.wfkind;
+--             apply HsJudgment.ax;
+--             {apply HsJudgment.wfctor;
+--               {
+--         apply HsJudgment.allt
+--         · apply HsJudgment.ax
+--           apply HsJudgment.wfdatatype
+--           · apply HsJudgment.arrowk
+--             · apply HsJudgment.ax
+--               apply HsJudgment.wfnil
+--             · apply HsJudgment.ax
+--               apply HsJudgment.wfnil
+--           · apply HsJudgment.wfnil
+--         · apply HsJudgment.arrow
+--           · apply HsJudgment.varTy
+--             · apply HsJudgment.wfkind
+--               · apply HsJudgment.ax
+--                 apply HsJudgment.wfdatatype
+--                 · apply HsJudgment.arrowk
+--                   · apply HsJudgment.ax
+--                     apply HsJudgment.wfnil
+--                   · apply HsJudgment.ax
+--                     apply HsJudgment.wfnil
+--                 · apply HsJudgment.wfnil
+--               · apply HsJudgment.wfdatatype
+--                 · apply HsJudgment.arrowk
+--                   · apply HsJudgment.ax
+--                     apply HsJudgment.wfnil
+--                   · apply HsJudgment.ax
+--                     apply HsJudgment.wfnil
+--                 · apply HsJudgment.wfnil
+--             · simp_all only [dnth, substType_HsTerm, Bool.or_eq_true]
+--               apply Or.inr
+--               rfl
+--             · simp_all only [dnth, substType_HsTerm, Frame.get_type_apply_commute]
+--               rfl
+--           · apply HsJudgment.appk
+--             on_goal 2 => {
+--               apply HsJudgment.varTy
+--               · apply HsJudgment.wfempty
+--                 apply HsJudgment.wfkind
+--                 · apply HsJudgment.ax
+--                   apply HsJudgment.wfdatatype
+--                   · apply HsJudgment.arrowk
+--                     · apply HsJudgment.ax
+--                       apply HsJudgment.wfnil
+--                     · apply HsJudgment.ax
+--                       apply HsJudgment.wfnil
+--                   · apply HsJudgment.wfnil
+--                 · apply HsJudgment.wfdatatype
+--                   · apply HsJudgment.arrowk
+--                     · apply HsJudgment.ax
+--                       apply HsJudgment.wfnil
+--                     · apply HsJudgment.ax
+--                       apply HsJudgment.wfnil
+--                   · apply HsJudgment.wfnil
+--               · simp_all only [dnth, substType_HsTerm, Bool.or_eq_true]
+--                 apply Or.inr
+--                 rfl
+--               · simp_all only [dnth, substType_HsTerm, Frame.get_type_apply_commute, Option.map_map]
+--                 rfl
+--             }
+--             · simp_all only [Function.comp_apply, HsTerm.subst_const]
+--               apply HsJudgment.varTy
+--               · apply HsJudgment.wfempty
+--                 apply HsJudgment.wfkind
+--                 · apply HsJudgment.ax
+--                   apply HsJudgment.wfdatatype
+--                   · apply HsJudgment.arrowk
+--                     · apply HsJudgment.ax
+--                       apply HsJudgment.wfnil
+--                     · apply HsJudgment.ax
+--                       apply HsJudgment.wfnil
+--                   · apply HsJudgment.wfnil
+--                 · apply HsJudgment.wfdatatype
+--                   · apply HsJudgment.arrowk
+--                     · apply HsJudgment.ax
+--                       apply HsJudgment.wfnil
+--                     · apply HsJudgment.ax
+--                       apply HsJudgment.wfnil
+--                   · apply HsJudgment.wfnil
+--               · simp_all only [dnth, substType_HsTerm, Bool.or_eq_true]
+--                 apply Or.inl
+--                 rfl
+--               · simp_all only [dnth, substType_HsTerm, Frame.get_type_apply_commute, Option.map_map]
+--                 rfl};
+--               apply HsJudgment.wfdatatype;
+--               apply HsJudgment.arrowk;
+--               apply HsJudgment.ax;
+--               apply HsJudgment.wfnil;
+--               apply HsJudgment.ax;
+--               apply HsJudgment.wfnil;
+--               apply HsJudgment.wfnil;
+--               {
+--                 apply ValidHsCtorType.all; apply ValidHsCtorType.arrow;
+--                 apply ValidHsCtorType.refl; unfold HsValidHeadVariable; simp;
+--                 simp_all only [Frame.apply, Frame.is_datatype];
+--               }
+--             };
+--             { apply HsJudgment.wfctor;
+--               {
+--         apply HsJudgment.allt
+--         · apply HsJudgment.ax
+--           apply HsJudgment.wfdatatype
+--           · apply HsJudgment.arrowk
+--             · apply HsJudgment.ax
+--               apply HsJudgment.wfnil
+--             · apply HsJudgment.ax
+--               apply HsJudgment.wfnil
+--           · apply HsJudgment.wfnil
+--         · apply HsJudgment.arrow
+--           · apply HsJudgment.varTy
+--             · apply HsJudgment.wfkind
+--               · apply HsJudgment.ax
+--                 apply HsJudgment.wfdatatype
+--                 · apply HsJudgment.arrowk
+--                   · apply HsJudgment.ax
+--                     apply HsJudgment.wfnil
+--                   · apply HsJudgment.ax
+--                     apply HsJudgment.wfnil
+--                 · apply HsJudgment.wfnil
+--               · apply HsJudgment.wfdatatype
+--                 · apply HsJudgment.arrowk
+--                   · apply HsJudgment.ax
+--                     apply HsJudgment.wfnil
+--                   · apply HsJudgment.ax
+--                     apply HsJudgment.wfnil
+--                 · apply HsJudgment.wfnil
+--             · simp_all only [dnth, substType_HsTerm, Bool.or_eq_true]
+--               apply Or.inr
+--               rfl
+--             · simp_all only [dnth, substType_HsTerm, Frame.get_type_apply_commute]
+--               rfl
+--           · apply HsJudgment.appk
+--             on_goal 2 => {
+--               apply HsJudgment.varTy
+--               · apply HsJudgment.wfempty
+--                 apply HsJudgment.wfkind
+--                 · apply HsJudgment.ax
+--                   apply HsJudgment.wfdatatype
+--                   · apply HsJudgment.arrowk
+--                     · apply HsJudgment.ax
+--                       apply HsJudgment.wfnil
+--                     · apply HsJudgment.ax
+--                       apply HsJudgment.wfnil
+--                   · apply HsJudgment.wfnil
+--                 · apply HsJudgment.wfdatatype
+--                   · apply HsJudgment.arrowk
+--                     · apply HsJudgment.ax
+--                       apply HsJudgment.wfnil
+--                     · apply HsJudgment.ax
+--                       apply HsJudgment.wfnil
+--                   · apply HsJudgment.wfnil
+--               · simp_all only [dnth, substType_HsTerm, Bool.or_eq_true]
+--                 apply Or.inr
+--                 rfl
+--               · simp_all only [dnth, substType_HsTerm, Frame.get_type_apply_commute, Option.map_map]
+--                 rfl
+--             }
+--             · simp_all only [Function.comp_apply, HsTerm.subst_const]
+--               apply HsJudgment.varTy
+--               · apply HsJudgment.wfempty
+--                 apply HsJudgment.wfkind
+--                 · apply HsJudgment.ax
+--                   apply HsJudgment.wfdatatype
+--                   · apply HsJudgment.arrowk
+--                     · apply HsJudgment.ax
+--                       apply HsJudgment.wfnil
+--                     · apply HsJudgment.ax
+--                       apply HsJudgment.wfnil
+--                   · apply HsJudgment.wfnil
+--                 · apply HsJudgment.wfdatatype
+--                   · apply HsJudgment.arrowk
+--                     · apply HsJudgment.ax
+--                       apply HsJudgment.wfnil
+--                     · apply HsJudgment.ax
+--                       apply HsJudgment.wfnil
+--                   · apply HsJudgment.wfnil
+--               · simp_all only [dnth, substType_HsTerm, Bool.or_eq_true]
+--                 apply Or.inl
+--                 rfl
+--               · simp_all only [dnth, substType_HsTerm, Frame.get_type_apply_commute, Option.map_map]
+--                 rfl
+--               };
+--               { apply HsJudgment.wfdatatype
+--                 · apply HsJudgment.arrowk
+--                   · apply HsJudgment.ax
+--                     apply HsJudgment.wfnil
+--                   · apply HsJudgment.ax
+--                     apply HsJudgment.wfnil
+--                 · apply HsJudgment.wfnil };
+--               {
+--                 apply ValidHsCtorType.all; apply ValidHsCtorType.arrow;
+--                 apply ValidHsCtorType.refl; unfold HsValidHeadVariable; simp;
+--                 simp_all only [Frame.apply, Frame.is_datatype]
+--               }
+--           }};
+--           { simp_all only [dnth, substType_HsTerm, Bool.or_eq_true]; apply Or.inr; rfl};
+--           { simp_all only [dnth, substType_HsTerm, Bool.or_eq_true]; rfl };
+--           {
+--             sorry
+--           };
+--           {
+--             sorry
+--           }
+--     ⟩
 
-              };
-              {
-                apply HsJudgment.wfdatatype
-                · apply HsJudgment.arrowk
-                  · apply HsJudgment.ax
-                    apply HsJudgment.wfnil
-                  · apply HsJudgment.ax
-                    apply HsJudgment.wfnil
-                · apply HsJudgment.wfnil
-              };
-              {
-                apply ValidHsCtorType.all; apply ValidHsCtorType.arrow;
-                apply ValidHsCtorType.refl; unfold HsValidHeadVariable; simp;
-                simp_all only [Frame.apply, Frame.is_datatype];
-              };
+-- #eval compile_ctx MaybeCtx
+-- #guard compile_ctx MaybeCtx == .some [ .ctor (∀[★](#2 `@k #0))
+--                                      , .ctor (∀[★]#0 -t> (#2 `@k #1))
+--                                      , .datatype (★ -k> ★) ]
 
-            };
-            apply HsJudgment.wfctor;
-            apply HsJudgment.allt;
-            {
-                apply HsJudgment.ax
-                apply HsJudgment.wfdatatype
-                · apply HsJudgment.arrowk
-                  · apply HsJudgment.ax
-                    apply HsJudgment.wfnil
-                  · apply HsJudgment.ax
-                    apply HsJudgment.wfnil
-                · apply HsJudgment.wfnil
-            };
-            {
-                apply HsJudgment.arrow
-                · apply HsJudgment.varTy
-                  · apply HsJudgment.wfkind
-                    · apply HsJudgment.ax
-                      apply HsJudgment.wfdatatype
-                      · apply HsJudgment.arrowk
-                        · apply HsJudgment.ax
-                          apply HsJudgment.wfnil
-                        · apply HsJudgment.ax
-                          apply HsJudgment.wfnil
-                      · apply HsJudgment.wfnil
-                    · apply HsJudgment.wfdatatype
-                      · apply HsJudgment.arrowk
-                        · apply HsJudgment.ax
-                          apply HsJudgment.wfnil
-                        · apply HsJudgment.ax
-                          apply HsJudgment.wfnil
-                      · apply HsJudgment.wfnil
-                  · simp_all only [dnth, substType_HsTerm, Bool.or_eq_true]
-                    apply Or.inr
-                    rfl
-                  · simp_all only [dnth, substType_HsTerm, Frame.get_type_apply_commute]
-                    rfl
-                · apply HsJudgment.appk
-                  · apply HsJudgment.varTy
-                    · apply HsJudgment.wfempty
-                      apply HsJudgment.wfkind
-                      · apply HsJudgment.ax
-                        apply HsJudgment.wfdatatype
-                        · apply HsJudgment.arrowk
-                          · apply HsJudgment.ax
-                            apply HsJudgment.wfnil
-                          · apply HsJudgment.ax
-                            apply HsJudgment.wfnil
-                        · apply HsJudgment.wfnil
-                      · apply HsJudgment.wfdatatype
-                        · apply HsJudgment.arrowk
-                          · apply HsJudgment.ax
-                            apply HsJudgment.wfnil
-                          · apply HsJudgment.ax
-                            apply HsJudgment.wfnil
-                        · apply HsJudgment.wfnil
-                    · simp_all only [dnth, substType_HsTerm, Bool.or_eq_true]
-                      apply Or.inl
-                      rfl
-                    · simp_all only [dnth, substType_HsTerm, Frame.get_type_apply_commute, Option.map_map]
-                      rfl
-                  · simp_all only [HsTerm.smap, HsTerm.smap.eq_3]
-                    apply HsJudgment.varTy
-                    · apply HsJudgment.wfempty
-                      apply HsJudgment.wfkind
-                      · apply HsJudgment.ax
-                        apply HsJudgment.wfdatatype
-                        · apply HsJudgment.arrowk
-                          · apply HsJudgment.ax
-                            apply HsJudgment.wfnil
-                          · apply HsJudgment.ax
-                            apply HsJudgment.wfnil
-                        · apply HsJudgment.wfnil
-                      · apply HsJudgment.wfdatatype
-                        · apply HsJudgment.arrowk
-                          · apply HsJudgment.ax
-                            apply HsJudgment.wfnil
-                          · apply HsJudgment.ax
-                            apply HsJudgment.wfnil
-                        · apply HsJudgment.wfnil
-                    · simp_all only [dnth, substType_HsTerm, Bool.or_eq_true]
-                      apply Or.inr
-                      rfl
-                    · simp_all only [dnth, substType_HsTerm, Frame.get_type_apply_commute, Option.map_map]
-                      rfl
-            };
-            apply HsJudgment.wfdatatype;
-            apply HsJudgment.arrowk;
-            apply HsJudgment.ax; apply HsJudgment.wfnil;
-            apply HsJudgment.ax; apply HsJudgment.wfnil;
-            apply HsJudgment.wfnil;
-            apply ValidHsCtorType.all; apply ValidHsCtorType.arrow;
-            apply ValidHsCtorType.refl; unfold HsValidHeadVariable; simp;
-            simp_all only [Frame.apply, Frame.is_datatype];
-          simp; apply Or.inl; rfl;
-          unfold Frame.get_type; unfold dnth; unfold Frame.apply; unfold dnth;
-          simp; unfold Frame.apply; simp; rfl;
-        apply HsJudgment.varTy;
-          {apply HsJudgment.wfkind;
-            apply HsJudgment.ax;
-            {apply HsJudgment.wfctor;
-              {
-        apply HsJudgment.allt
-        · apply HsJudgment.ax
-          apply HsJudgment.wfdatatype
-          · apply HsJudgment.arrowk
-            · apply HsJudgment.ax
-              apply HsJudgment.wfnil
-            · apply HsJudgment.ax
-              apply HsJudgment.wfnil
-          · apply HsJudgment.wfnil
-        · apply HsJudgment.arrow
-          · apply HsJudgment.varTy
-            · apply HsJudgment.wfkind
-              · apply HsJudgment.ax
-                apply HsJudgment.wfdatatype
-                · apply HsJudgment.arrowk
-                  · apply HsJudgment.ax
-                    apply HsJudgment.wfnil
-                  · apply HsJudgment.ax
-                    apply HsJudgment.wfnil
-                · apply HsJudgment.wfnil
-              · apply HsJudgment.wfdatatype
-                · apply HsJudgment.arrowk
-                  · apply HsJudgment.ax
-                    apply HsJudgment.wfnil
-                  · apply HsJudgment.ax
-                    apply HsJudgment.wfnil
-                · apply HsJudgment.wfnil
-            · simp_all only [dnth, substType_HsTerm, Bool.or_eq_true]
-              apply Or.inr
-              rfl
-            · simp_all only [dnth, substType_HsTerm, Frame.get_type_apply_commute]
-              rfl
-          · apply HsJudgment.appk
-            on_goal 2 => {
-              apply HsJudgment.varTy
-              · apply HsJudgment.wfempty
-                apply HsJudgment.wfkind
-                · apply HsJudgment.ax
-                  apply HsJudgment.wfdatatype
-                  · apply HsJudgment.arrowk
-                    · apply HsJudgment.ax
-                      apply HsJudgment.wfnil
-                    · apply HsJudgment.ax
-                      apply HsJudgment.wfnil
-                  · apply HsJudgment.wfnil
-                · apply HsJudgment.wfdatatype
-                  · apply HsJudgment.arrowk
-                    · apply HsJudgment.ax
-                      apply HsJudgment.wfnil
-                    · apply HsJudgment.ax
-                      apply HsJudgment.wfnil
-                  · apply HsJudgment.wfnil
-              · simp_all only [dnth, substType_HsTerm, Bool.or_eq_true]
-                apply Or.inr
-                rfl
-              · simp_all only [dnth, substType_HsTerm, Frame.get_type_apply_commute, Option.map_map]
-                rfl
-            }
-            · simp_all only [Function.comp_apply, HsTerm.subst_const]
-              apply HsJudgment.varTy
-              · apply HsJudgment.wfempty
-                apply HsJudgment.wfkind
-                · apply HsJudgment.ax
-                  apply HsJudgment.wfdatatype
-                  · apply HsJudgment.arrowk
-                    · apply HsJudgment.ax
-                      apply HsJudgment.wfnil
-                    · apply HsJudgment.ax
-                      apply HsJudgment.wfnil
-                  · apply HsJudgment.wfnil
-                · apply HsJudgment.wfdatatype
-                  · apply HsJudgment.arrowk
-                    · apply HsJudgment.ax
-                      apply HsJudgment.wfnil
-                    · apply HsJudgment.ax
-                      apply HsJudgment.wfnil
-                  · apply HsJudgment.wfnil
-              · simp_all only [dnth, substType_HsTerm, Bool.or_eq_true]
-                apply Or.inl
-                rfl
-              · simp_all only [dnth, substType_HsTerm, Frame.get_type_apply_commute, Option.map_map]
-                rfl};
-              apply HsJudgment.wfdatatype;
-              apply HsJudgment.arrowk;
-              apply HsJudgment.ax;
-              apply HsJudgment.wfnil;
-              apply HsJudgment.ax;
-              apply HsJudgment.wfnil;
-              apply HsJudgment.wfnil;
-              {
-                apply ValidHsCtorType.all; apply ValidHsCtorType.arrow;
-                apply ValidHsCtorType.refl; unfold HsValidHeadVariable; simp;
-                simp_all only [Frame.apply, Frame.is_datatype];
-              }
-            };
-            { apply HsJudgment.wfctor;
-              {
-
-        apply HsJudgment.allt
-        · apply HsJudgment.ax
-          apply HsJudgment.wfdatatype
-          · apply HsJudgment.arrowk
-            · apply HsJudgment.ax
-              apply HsJudgment.wfnil
-            · apply HsJudgment.ax
-              apply HsJudgment.wfnil
-          · apply HsJudgment.wfnil
-        · apply HsJudgment.arrow
-          · apply HsJudgment.varTy
-            · apply HsJudgment.wfkind
-              · apply HsJudgment.ax
-                apply HsJudgment.wfdatatype
-                · apply HsJudgment.arrowk
-                  · apply HsJudgment.ax
-                    apply HsJudgment.wfnil
-                  · apply HsJudgment.ax
-                    apply HsJudgment.wfnil
-                · apply HsJudgment.wfnil
-              · apply HsJudgment.wfdatatype
-                · apply HsJudgment.arrowk
-                  · apply HsJudgment.ax
-                    apply HsJudgment.wfnil
-                  · apply HsJudgment.ax
-                    apply HsJudgment.wfnil
-                · apply HsJudgment.wfnil
-            · simp_all only [dnth, substType_HsTerm, Bool.or_eq_true]
-              apply Or.inr
-              rfl
-            · simp_all only [dnth, substType_HsTerm, Frame.get_type_apply_commute]
-              rfl
-          · apply HsJudgment.appk
-            on_goal 2 => {
-              apply HsJudgment.varTy
-              · apply HsJudgment.wfempty
-                apply HsJudgment.wfkind
-                · apply HsJudgment.ax
-                  apply HsJudgment.wfdatatype
-                  · apply HsJudgment.arrowk
-                    · apply HsJudgment.ax
-                      apply HsJudgment.wfnil
-                    · apply HsJudgment.ax
-                      apply HsJudgment.wfnil
-                  · apply HsJudgment.wfnil
-                · apply HsJudgment.wfdatatype
-                  · apply HsJudgment.arrowk
-                    · apply HsJudgment.ax
-                      apply HsJudgment.wfnil
-                    · apply HsJudgment.ax
-                      apply HsJudgment.wfnil
-                  · apply HsJudgment.wfnil
-              · simp_all only [dnth, substType_HsTerm, Bool.or_eq_true]
-                apply Or.inr
-                rfl
-              · simp_all only [dnth, substType_HsTerm, Frame.get_type_apply_commute, Option.map_map]
-                rfl
-            }
-            · simp_all only [Function.comp_apply, HsTerm.subst_const]
-              apply HsJudgment.varTy
-              · apply HsJudgment.wfempty
-                apply HsJudgment.wfkind
-                · apply HsJudgment.ax
-                  apply HsJudgment.wfdatatype
-                  · apply HsJudgment.arrowk
-                    · apply HsJudgment.ax
-                      apply HsJudgment.wfnil
-                    · apply HsJudgment.ax
-                      apply HsJudgment.wfnil
-                  · apply HsJudgment.wfnil
-                · apply HsJudgment.wfdatatype
-                  · apply HsJudgment.arrowk
-                    · apply HsJudgment.ax
-                      apply HsJudgment.wfnil
-                    · apply HsJudgment.ax
-                      apply HsJudgment.wfnil
-                  · apply HsJudgment.wfnil
-              · simp_all only [dnth, substType_HsTerm, Bool.or_eq_true]
-                apply Or.inl
-                rfl
-              · simp_all only [dnth, substType_HsTerm, Frame.get_type_apply_commute, Option.map_map]
-                rfl
-              };
-              { apply HsJudgment.wfdatatype
-                · apply HsJudgment.arrowk
-                  · apply HsJudgment.ax
-                    apply HsJudgment.wfnil
-                  · apply HsJudgment.ax
-                    apply HsJudgment.wfnil
-                · apply HsJudgment.wfnil };
-              {
-                apply ValidHsCtorType.all; apply ValidHsCtorType.arrow;
-                apply ValidHsCtorType.refl; unfold HsValidHeadVariable; simp;
-                simp_all only [Frame.apply, Frame.is_datatype]
-              }
-          }};
-          { simp_all only [dnth, substType_HsTerm, Bool.or_eq_true]; apply Or.inr; rfl};
-          {simp_all only [dnth, substType_HsTerm, Bool.or_eq_true]; rfl};
-    ⟩
-
-#eval compile_ctx MaybeCtx
-#guard compile_ctx MaybeCtx == .some [ .ctor (∀[★](#2 `@k #0))
-                                     , .ctor (∀[★]#0 -t> (#2 `@k #1))
-                                     , .datatype (★ -k> ★) ]
-
-#guard compile .ctx MbCtx MaybeCtx == compile_ctx MaybeCtx
+-- #guard compile .ctx MbCtx MaybeCtx == compile_ctx MaybeCtx
 #guard compile .type [] ⟨(idHsType, `★), idTypeKinding⟩ == compile_type [] idHsType `★ idTypeKinding
 #guard compile .term [] ⟨(idHsTerm, idHsType), idTyping⟩ == compile_term [] idHsTerm idHsType idTyping
