Hs/Metatheory/SubstitutionCompile.lean
@@ -1,0 +1,16 @@
+import Hs.HsTerm
+import Hs.HsJudgment
+import SystemFD.Ctx
+import Hs.Metatheory.TypeMatch
+import Hs.Metatheory.Weaken
+import Hs.Metatheory.WeakenCompile
+import Hs.Metatheory.Substitution
+import Hs.Algorithm
+
+theorem compile_beta_kind_type :
+  (j1 : (.kind A::Γ) ⊢τ b : B) ->
+  compile_type (.kind A::Γ) b B j1 = .some b' ->
+  (j2 : Γ ⊢τ t : A) ->
+  compile_type Γ t A j2 = .some t' ->
+  (j3 : Γ ⊢τ (b β[t]) : (B β[t])) ->
+  compile_type Γ (b β[t]) (B β[t]) j3 = .some (b' β[t']) := by sorry
