Hs/Metatheory/WeakenCompile.lean
@@ -1,0 +1,70 @@
+import Hs.HsTerm
+import Hs.HsJudgment
+import SystemFD.Ctx
+import Hs.Algorithm
+
+set_option maxHeartbeats 1000000
+
+theorem weaken_compile_kind :
+  (j : Γ ⊢κ t : k) ->
+  (sj : (f :: Γ) ⊢κ ([S]t) : ([S]k)) ->
+  compile_kind Γ t k j = .some t' ->
+  compile_kind (f::Γ) ([S]t) ([S]k) sj = .some ([S]t') := by
+intro j sj c;
+induction Γ, t, k, j using compile_kind.induct generalizing t';
+case _ =>
+  unfold compile_kind; cases sj; simp; unfold compile_kind at c; cases c; simp;
+case _ j1 j2 ih1 ih2 =>
+  unfold compile_kind at c; simp at c;
+  rw[Option.bind_eq_some] at c;
+  cases c; case _ wa c =>
+  cases c; case _ ca cb =>
+  rw[Option.bind_eq_some] at cb;
+  cases cb; case _ wb cb =>
+  cases cb; case _ cb e =>
+  cases e; cases sj;
+  case _ jaw jbw =>
+  have ih1' := @ih1 wa jaw ca
+  have ih2' := @ih2 wb jbw cb
+  unfold compile_kind; simp;
+  rw[Option.bind_eq_some];
+  exists ([S]wa); apply And.intro;
+  assumption;
+  rw[Option.bind_eq_some];
+  exists ([S]wb);
+
+
+theorem weaken_compile_type :
+  (j : Γ ⊢τ t : k) ->
+  (sj : (f :: Γ) ⊢τ ([S]t) : ([S]k)) ->
+  compile_type Γ t k j = .some t' ->
+  compile_type (f::Γ) ([S]t) ([S]k) sj = .some ([S]t') := by
+intro j sj c;
+induction Γ, t, k, j using compile_type.induct generalizing t' <;> simp at *;
+case _ =>
+  unfold compile_type; cases sj; simp; unfold compile_type at c; cases c; simp
+case _ => sorry
+case _ => sorry
+case _ j1 j2 ih1 ih2 =>
+  unfold compile_type at c; simp at c;
+  rw[Option.bind_eq_some] at c;
+  cases c; case _ wa c =>
+  cases c; case _ ca cb =>
+  rw[Option.bind_eq_some] at cb;
+  cases cb; case _ wb cb =>
+  cases cb; case _ cb e =>
+  cases e;
+  cases sj; case _ ja jb =>
+  unfold compile_type; simp;
+
+  rw[Option.bind_eq_some];
+  exists ([S]wa);
+  apply And.intro;
+  case _ ja =>
+    sorry
+  rw[Option.bind_eq_some];
+  exists ([^S]wb)
+  apply And.intro
+  sorry
+  simp
+case _ => sorry
