SystemFD/Ctx.lean
@@ -331,6 +331,14 @@ namespace Ctx
 end Ctx
 
 omit [Repr T] [Inhabited T] [SubstitutionTypeLaws T]
+theorem kind_indexing_exists {Γ : Ctx T} :
+  (Γ d@ n).is_kind = true ->
+  ∃ t, Γ d@ n = .kind t := by
+intros h; unfold Frame.is_kind at h; split at h;
+case _ a h' => apply Exists.intro a; assumption
+case _ => cases h
+
+omit [Repr T] [Inhabited T] [SubstitutionTypeLaws T]
 theorem datatype_indexing_exists {Γ : Ctx T} :
   (Γ d@ n).is_datatype = true ->
   ∃ t, Γ d@ n = .datatype t := by
